NuSys.thy
@@ -1,9 +1,9 @@
 theory NuSys
   imports NuPrime "HOL-Eisbach.Eisbach" "HOL-Eisbach.Eisbach_Tools"
   keywords
-    "proc" "rec_proc" "\<phi>cast" :: thy_goal_stmt
-  and "as" "\<rightarrow>" "\<longmapsto>" "\<leftarrow>" "^" "^*" "requires" "\<Longleftarrow>" "\<Longleftarrow>'" "$"
-    "var" "always"  "\<medium_left_bracket>" "\<medium_right_bracket>" "\<Longrightarrow>" "goal" "\<exists>" "heap" "stack"
+    "proc" "rec_proc" (*"\<phi>cast"*) :: thy_goal_stmt
+  and "as" "\<rightarrow>" "\<longmapsto>" "\<leftarrow>" "^" "^*" "\<Longleftarrow>" "\<Longleftarrow>'" "$"
+    "var" "always" "\<Longrightarrow>" "goal" "\<exists>" "heap" "stack"
     "argument" "return" "on" "affirm" "no" :: quasi_command
   and ";;" "\<medium_left_bracket>" "\<medium_right_bracket>" :: prf_decl % "proof"
   and "\<phi>processor" "\<phi>reasoner" "\<phi>reasoner_ML" :: thy_decl % "ML"
@@ -19,18 +19,13 @@ abbrevs
   and "<label>" = "\<^bold>l\<^bold>a\<^bold>b\<^bold>e\<^bold>l"
   and "<index>" = "\<^bold>i\<^bold>n\<^bold>d\<^bold>e\<^bold>x"
       and "as" = "\<^bold>a\<^bold>s"
-      and "<at>" = "\<^bold>a\<^bold>t"
       and "<and>" = "\<^bold>a\<^bold>n\<^bold>d"
-      and "in" = "\<^bold>i\<^bold>n"
       and "<with>" = "\<^bold>w\<^bold>i\<^bold>t\<^bold>h"
       and "<facts>" = "\<^bold>f\<^bold>a\<^bold>c\<^bold>t\<^bold>s"
       and "<proc>" = "\<^bold>p\<^bold>r\<^bold>o\<^bold>c"
       and "<func>" = "\<^bold>f\<^bold>u\<^bold>n\<^bold>c"
       and "<map>" = "\<^bold>m\<^bold>a\<^bold>p"
       and "<subty>" = "\<^bold>s\<^bold>u\<^bold>b\<^bold>t\<^bold>y\<^bold>p\<^bold>e"
-      and "<make>" = "\<^bold>m\<^bold>a\<^bold>k\<^bold>e"
-      and "<auto>" = "\<^bold>a\<^bold>u\<^bold>t\<^bold>o"
-      and "<construct>" = "\<^bold>c\<^bold>o\<^bold>n\<^bold>s\<^bold>t\<^bold>r\<^bold>u\<^bold>c\<^bold>t"
       and "<by>" = "\<^bold>b\<^bold>y"
       and "<simplify>" = "\<^bold>s\<^bold>i\<^bold>m\<^bold>p\<^bold>l\<^bold>i\<^bold>f\<^bold>y"
       and "<heap>" = "\<^bold>h\<^bold>e\<^bold>a\<^bold>p"
@@ -39,13 +34,11 @@ abbrevs
       and "<when>" = "\<^bold>w\<^bold>h\<^bold>e\<^bold>n"
       and "<dest>" = "\<^bold>d\<^bold>e\<^bold>s\<^bold>t"
       and "<try>" = "\<^bold>t\<^bold>r\<^bold>y"
-  and "<get>" = "\<^bold>g\<^bold>e\<^bold>t"
-  and "<map>" = "\<^bold>m\<^bold>a\<^bold>p"
-  and "<field>" = "\<^bold>f\<^bold>i\<^bold>e\<^bold>l\<^bold>d"
   and "<obligation>" = "\<^bold>o\<^bold>b\<^bold>l\<^bold>i\<^bold>g\<^bold>a\<^bold>t\<^bold>i\<^bold>o\<^bold>n"
   and "<conv>" = "\<^bold>c\<^bold>o\<^bold>n\<^bold>v"
   and ">->" = "\<Zinj>"
   and "<;>" = "\<Zcomp>"
+  and "<@GOAL>" = "\<^bold>@\<^bold>G\<^bold>O\<^bold>A\<^bold>L"
 begin
 
 declare [ [ML_debugger, ML_exception_debugger] ]
@@ -184,6 +177,23 @@ definition \<phi>Equal :: "('VAL,'a) \<phi> \<Rightarrow> ('a \<Rightarrow> 'a \
 
 end
 
+definition Subty :: " 'a set \<Rightarrow> 'a set \<Rightarrow> bool \<Rightarrow> bool " ("(2\<^bold>s\<^bold>u\<^bold>b\<^bold>t\<^bold>y\<^bold>p\<^bold>e _/ \<longmapsto> _/ \<^bold>w\<^bold>i\<^bold>t\<^bold>h _)" [13,13,13] 12)
+  where "(\<^bold>s\<^bold>u\<^bold>b\<^bold>t\<^bold>y\<^bold>p\<^bold>e A \<longmapsto> B \<^bold>w\<^bold>i\<^bold>t\<^bold>h P) \<longleftrightarrow> (\<forall>v. v \<in> A \<longrightarrow> v \<in> B \<and> P)"
+
+lemma (in std) \<phi>CONSEQ_left:
+  \<open>\<^bold>s\<^bold>u\<^bold>b\<^bold>t\<^bold>y\<^bold>p\<^bold>e X \<longmapsto> X' \<^bold>w\<^bold>i\<^bold>t\<^bold>h P
+\<Longrightarrow> \<^bold>p\<^bold>r\<^bold>o\<^bold>c f \<lbrace> X' \<longmapsto> Y \<rbrace>
+\<Longrightarrow> \<^bold>p\<^bold>r\<^bold>o\<^bold>c f \<lbrace> X \<longmapsto> Y \<rbrace>\<close>
+  unfolding Subty_def \<phi>Procedure_def
+  by (smt (z3) mem_Collect_eq set_mult_expn std.INTERP_COMP_def std_axioms)
+
+lemma (in std) \<phi>CONSEQ_right:
+  \<open>\<^bold>s\<^bold>u\<^bold>b\<^bold>t\<^bold>y\<^bold>p\<^bold>e Y \<longmapsto> Y' \<^bold>w\<^bold>i\<^bold>t\<^bold>h P
+\<Longrightarrow> \<^bold>p\<^bold>r\<^bold>o\<^bold>c f \<lbrace> X \<longmapsto> Y \<rbrace>
+\<Longrightarrow> \<^bold>p\<^bold>r\<^bold>o\<^bold>c f \<lbrace> X \<longmapsto> Y' \<rbrace>\<close>
+  unfolding Subty_def \<phi>Procedure_def
+  by (smt (z3) INTERP_COMP_def LooseStateTy_expn' mem_Collect_eq set_mult_expn)
+
 
 subsubsection \<open>Elementary\<close>
 
@@ -307,6 +317,11 @@ end\<close>
 declare conjI[\<phi>reason] TrueI[\<phi>reason] set_mult_inhabited[\<phi>reason_elim!]
 
 declare (in std) Obj_Ele_inhabited[\<phi>reason_elim!] Val_Ele_inhabited[\<phi>reason_elim!]
+
+lemma (in std) [\<phi>reason]:
+  \<open> (\<And>x. \<phi>SemType (x \<Ztypecolon> T) TY)
+\<Longrightarrow> \<phi>\<phi>SemType T TY\<close>
+  ..
 
 subsection \<open>Tags - Part I\<close>
 
@@ -514,7 +529,7 @@ text \<open>Sequent in pattern \<^prop>\<open>\<^bold>a\<^bold>r\<^bold>g\<^bold
 
 subsubsection \<open>Reasoning Helpers\<close>
 
-definition Subty_Target :: " 'a \<Rightarrow> 'a "  ("\<medium_left_bracket> _ \<medium_right_bracket>") where "\<medium_left_bracket> x \<medium_right_bracket> = x"
+definition FOCUS_TAG :: " 'a \<Rightarrow> 'a "  ("\<blangle> _ \<brangle>") where [iff]: "\<blangle> x \<brangle> = x"
 
 
 subsubsection \<open>Technical Tags\<close>
@@ -579,9 +594,6 @@ subsection \<open>Subtype & View Shift\<close>
 
 paragraph \<open>Definitions\<close>
 
-definition Subty :: " 'a set \<Rightarrow> 'a set \<Rightarrow> bool \<Rightarrow> bool " ("(2\<^bold>s\<^bold>u\<^bold>b\<^bold>t\<^bold>y\<^bold>p\<^bold>e _/ \<longmapsto> _/ \<^bold>w\<^bold>i\<^bold>t\<^bold>h _)" [13,13,13] 12)
-  where "(\<^bold>s\<^bold>u\<^bold>b\<^bold>t\<^bold>y\<^bold>p\<^bold>e A \<longmapsto> B \<^bold>w\<^bold>i\<^bold>t\<^bold>h P) \<longleftrightarrow> (\<forall>v. v \<in> A \<longrightarrow> v \<in> B \<and> P)"
-
 consts SimpleSubty :: " 'a set \<Rightarrow> 'a set \<Rightarrow> bool \<Rightarrow> bool " ("(2\<^bold>s\<^bold>u\<^bold>b\<^bold>t\<^bold>y\<^bold>p\<^bold>e _/ \<longmapsto> _)" [13,13] 12)
 translations "(\<^bold>s\<^bold>u\<^bold>b\<^bold>t\<^bold>y\<^bold>p\<^bold>e A \<longmapsto> B)" == "(\<^bold>s\<^bold>u\<^bold>b\<^bold>t\<^bold>y\<^bold>p\<^bold>e A \<longmapsto> B \<^bold>w\<^bold>i\<^bold>t\<^bold>h CONST True)"
 
@@ -630,12 +642,12 @@ lemma [\<phi>reason 2000]:
 
 lemma (in std) "\<phi>cast":
   "\<^bold>c\<^bold>u\<^bold>r\<^bold>r\<^bold>e\<^bold>n\<^bold>t blk [H] \<^bold>r\<^bold>e\<^bold>s\<^bold>u\<^bold>l\<^bold>t\<^bold>s \<^bold>i\<^bold>n T \<Longrightarrow> \<^bold>s\<^bold>u\<^bold>b\<^bold>t\<^bold>y\<^bold>p\<^bold>e T \<longmapsto> T' \<^bold>w\<^bold>i\<^bold>t\<^bold>h P \<Longrightarrow> \<^bold>c\<^bold>u\<^bold>r\<^bold>r\<^bold>e\<^bold>n\<^bold>t blk [H] \<^bold>r\<^bold>e\<^bold>s\<^bold>u\<^bold>l\<^bold>t\<^bold>s \<^bold>i\<^bold>n T'"
-  unfolding CurrentConstruction_def Subty_Target_def Subty_def
+  unfolding CurrentConstruction_def Subty_def
   by (cases blk, simp_all add: pair_All \<phi>expns) blast
 
 lemma (in std) "\<phi>cast_P":
   "\<^bold>c\<^bold>u\<^bold>r\<^bold>r\<^bold>e\<^bold>n\<^bold>t blk [H] \<^bold>r\<^bold>e\<^bold>s\<^bold>u\<^bold>l\<^bold>t\<^bold>s \<^bold>i\<^bold>n T \<Longrightarrow> \<^bold>s\<^bold>u\<^bold>b\<^bold>t\<^bold>y\<^bold>p\<^bold>e T \<longmapsto> T' \<^bold>w\<^bold>i\<^bold>t\<^bold>h P \<Longrightarrow> (\<^bold>c\<^bold>u\<^bold>r\<^bold>r\<^bold>e\<^bold>n\<^bold>t blk [H] \<^bold>r\<^bold>e\<^bold>s\<^bold>u\<^bold>l\<^bold>t\<^bold>s \<^bold>i\<^bold>n T') \<and> P"
-  unfolding CurrentConstruction_def Subty_Target_def Subty_def
+  unfolding CurrentConstruction_def Subty_def
   by (cases blk, simp_all add: pair_All \<phi>expns) blast
 
 lemma (in std) cast_val_\<phi>app[\<phi>overload cast]:
@@ -663,12 +675,6 @@ lemma cast_whole_\<phi>app:
   "\<^bold>a\<^bold>r\<^bold>g\<^bold>u\<^bold>m\<^bold>e\<^bold>n\<^bold>t \<^bold>s\<^bold>u\<^bold>b\<^bold>t\<^bold>y\<^bold>p\<^bold>e X \<longmapsto> X' \<^bold>w\<^bold>i\<^bold>t\<^bold>h P \<Longrightarrow> \<^bold>s\<^bold>u\<^bold>b\<^bold>t\<^bold>y\<^bold>p\<^bold>e X \<longmapsto> X' \<^bold>w\<^bold>i\<^bold>t\<^bold>h P"
   unfolding Subty_def Argument_def by (simp add: \<phi>expns)
 
-
-lemma cast_conversion:
-  "\<medium_left_bracket> \<^bold>s\<^bold>u\<^bold>b\<^bold>t\<^bold>y\<^bold>p\<^bold>e R \<longmapsto> T \<^bold>w\<^bold>i\<^bold>t\<^bold>h Q \<medium_right_bracket>
-  \<Longrightarrow> \<^bold>s\<^bold>u\<^bold>b\<^bold>t\<^bold>y\<^bold>p\<^bold>e T \<longmapsto> U \<^bold>w\<^bold>i\<^bold>t\<^bold>h P
-  \<Longrightarrow> \<^bold>s\<^bold>u\<^bold>b\<^bold>t\<^bold>y\<^bold>p\<^bold>e R \<longmapsto> U \<^bold>w\<^bold>i\<^bold>t\<^bold>h P \<and> Q"
-  unfolding Subty_Target_def Subty_def by blast
 
 
 (* lemma dual_cast_fallback[\<phi>intro']: "\<^bold>s\<^bold>u\<^bold>b\<^bold>t\<^bold>y\<^bold>p\<^bold>e A \<longmapsto> B \<^bold>w\<^bold>i\<^bold>t\<^bold>h P \<Longrightarrow> (\<^bold>s\<^bold>u\<^bold>b\<^bold>t\<^bold>y\<^bold>p\<^bold>e A \<longmapsto> B) \<and> (\<^bold>s\<^bold>u\<^bold>b\<^bold>t\<^bold>y\<^bold>p\<^bold>e C \<longmapsto> C)" unfolding Subty_def by fast *)
@@ -774,7 +780,8 @@ ML_file \<open>library/Subgoal_Env.ML\<close>
 \<phi>reasoner_ML CHK_SUBGOAL 2000 (conclusion \<open>CHK_SUBGOAL ?GOAL\<close>) = \<open>Subgoal_Env.chk_subgoal\<close>
 \<phi>reasoner_ML SOLVE_SUBGOAL 9999 (conclusion \<open>SOLVE_SUBGOAL ?GOAL\<close>) = \<open>Subgoal_Env.solve_subgoal\<close>
 
-definition Subty_Target2 :: " 'a \<Rightarrow> subgoal \<Rightarrow> 'a "  ("\<medium_left_bracket> _ \<medium_right_bracket>: _" [2,1000] 100) where "\<medium_left_bracket> x \<medium_right_bracket>: _ = x"
+definition GOAL_CTXT :: "bool \<Rightarrow> subgoal \<Rightarrow> prop"  ("_  \<^bold>@\<^bold>G\<^bold>O\<^bold>A\<^bold>L _" [2,1000] 2)
+  where [iff]: "GOAL_CTXT x _ \<equiv> Trueprop x"
 
 
 subsection \<open>Simplifier & Rewriter\<close>
@@ -851,7 +858,7 @@ lemma IntroFrameVar_Yes:
         Thm.major_prem_of sequent |> HOLogic.dest_Trueprop
     val tail = PhiSyntax.strip_separations S |> NuHelp.last
   in
-    if is_Var tail andalso fastype_of tail = \<^typ>\<open>('VAR,'FIC_N,'FIC)assn\<close>
+    if is_Var tail andalso fastype_of tail = PhiSyntax.get_assn_typ ctxt
     then Seq.single (ctxt, @{thm IntroFrameVar_No} RS sequent)
     else Seq.single (ctxt, @{thm IntroFrameVar_Yes} RS sequent)
   end\<close>
@@ -872,20 +879,20 @@ translations "SYNTHESIS (x \<Ztypecolon> T)" \<rightleftharpoons> "SYNTHESIS ELE
 lemma (in std) "__\<phi>synthesis__":
   " (\<^bold>c\<^bold>u\<^bold>r\<^bold>r\<^bold>e\<^bold>n\<^bold>t blk [H] \<^bold>r\<^bold>e\<^bold>s\<^bold>u\<^bold>l\<^bold>t\<^bold>s \<^bold>i\<^bold>n S1)
 \<Longrightarrow> SUBGOAL TOP_GOAL G
-\<Longrightarrow> \<medium_left_bracket> \<^bold>p\<^bold>r\<^bold>o\<^bold>c f \<lbrace> S1 \<longmapsto> S2\<heavy_comma> SYNTHESIS X \<rbrace> \<medium_right_bracket>: G
+\<Longrightarrow> \<^bold>p\<^bold>r\<^bold>o\<^bold>c f \<lbrace> S1 \<longmapsto> S2\<heavy_comma> SYNTHESIS X \<rbrace> \<^bold>@\<^bold>G\<^bold>O\<^bold>A\<^bold>L G
 \<Longrightarrow> \<r>Success
 \<Longrightarrow> \<^bold>o\<^bold>b\<^bold>l\<^bold>i\<^bold>g\<^bold>a\<^bold>t\<^bold>i\<^bold>o\<^bold>n True
 \<Longrightarrow> (\<^bold>p\<^bold>e\<^bold>n\<^bold>d\<^bold>i\<^bold>n\<^bold>g f \<^bold>o\<^bold>n blk [H] \<^bold>r\<^bold>e\<^bold>s\<^bold>u\<^bold>l\<^bold>t\<^bold>s \<^bold>i\<^bold>n S2\<heavy_comma> X)"
-  unfolding Synthesis_def Subty_Target2_def
+  unfolding Synthesis_def GOAL_CTXT_def
   using \<phi>apply_proc .
 
 
 subsection \<open>Application\<close> \<comment> \<open>of procedures, subtypings, and any other things\<close>
 
-definition \<phi>Application :: \<open>bool \<Rightarrow> bool \<Rightarrow> prop \<Rightarrow> prop\<close> ("_/ \<^bold>a\<^bold>p\<^bold>p\<^bold>l\<^bold>i\<^bold>e\<^bold>s _/ \<^bold>\<Rightarrow> _")
-  where \<open>\<phi>Application Applicants State Result \<equiv> (State \<Longrightarrow> Applicants \<Longrightarrow> PROP Result)\<close>
+definition \<phi>Application :: \<open>prop \<Rightarrow> bool \<Rightarrow> prop \<Rightarrow> prop\<close> ("_/ \<^bold>a\<^bold>p\<^bold>p\<^bold>l\<^bold>i\<^bold>e\<^bold>s _/ \<^bold>\<Rightarrow> _")
+  where \<open>\<phi>Application Applicants State Result \<equiv> (State \<Longrightarrow> PROP Applicants \<Longrightarrow> PROP Result)\<close>
 
-definition \<phi>Application_Method :: \<open>bool \<Rightarrow> bool \<Rightarrow> prop \<Rightarrow> prop\<close>
+definition \<phi>Application_Method :: \<open>prop \<Rightarrow> bool \<Rightarrow> prop \<Rightarrow> prop\<close>
   where \<open>\<phi>Application_Method \<equiv> \<phi>Application\<close>
 
 definition \<phi>Application_Success :: "prop"
@@ -898,17 +905,17 @@ definition \<phi>Application_Success :: "prop"
 
 
 lemma \<phi>Application_normalize:
-  \<open>(P \<Longrightarrow> Apps \<^bold>a\<^bold>p\<^bold>p\<^bold>l\<^bold>i\<^bold>e\<^bold>s State \<^bold>\<Rightarrow> (PROP Result))
- \<equiv> Apps \<^bold>a\<^bold>p\<^bold>p\<^bold>l\<^bold>i\<^bold>e\<^bold>s State \<^bold>\<Rightarrow> (P \<Longrightarrow> PROP Result)\<close>
+  \<open>(P \<Longrightarrow> ((PROP Apps) \<^bold>a\<^bold>p\<^bold>p\<^bold>l\<^bold>i\<^bold>e\<^bold>s State \<^bold>\<Rightarrow> (PROP Result)))
+ \<equiv> ((PROP Apps) \<^bold>a\<^bold>p\<^bold>p\<^bold>l\<^bold>i\<^bold>e\<^bold>s State \<^bold>\<Rightarrow> (P \<Longrightarrow> PROP Result))\<close>
   unfolding \<phi>Application_def ..
 
 lemma \<phi>application_start_reasoning:
-  \<open> PROP \<phi>Application_Method Apps State (PROP Result)
-\<Longrightarrow> Apps \<^bold>a\<^bold>p\<^bold>p\<^bold>l\<^bold>i\<^bold>e\<^bold>s State \<^bold>\<Rightarrow> (PROP Result)\<close>
+  \<open> PROP \<phi>Application_Method (PROP Apps) State (PROP Result)
+\<Longrightarrow> ((PROP Apps) \<^bold>a\<^bold>p\<^bold>p\<^bold>l\<^bold>i\<^bold>e\<^bold>s State \<^bold>\<Rightarrow> (PROP Result))\<close>
   unfolding \<phi>Application_def \<phi>Application_Method_def .
 
 lemma \<phi>application:
-  \<open>Apps \<Longrightarrow> State \<Longrightarrow> (Apps \<^bold>a\<^bold>p\<^bold>p\<^bold>l\<^bold>i\<^bold>e\<^bold>s State \<^bold>\<Rightarrow> (PROP Result)) \<Longrightarrow> PROP Pure.prop Result\<close>
+  \<open>PROP Apps \<Longrightarrow> State \<Longrightarrow> ((PROP Apps) \<^bold>a\<^bold>p\<^bold>p\<^bold>l\<^bold>i\<^bold>e\<^bold>s State \<^bold>\<Rightarrow> (PROP Result)) \<Longrightarrow> PROP Pure.prop Result\<close>
   unfolding \<phi>Application_def Pure.prop_def .
 
 lemma \<phi>application_success:
@@ -917,7 +924,7 @@ lemma \<phi>application_success:
 
 ML_file \<open>library/application.ML\<close>
 
-\<phi>reasoner_ML \<phi>Application 2000 (conclusion \<open>?App \<^bold>a\<^bold>p\<^bold>p\<^bold>l\<^bold>i\<^bold>e\<^bold>s ?State \<^bold>\<Rightarrow> (PROP ?Result)\<close>) =
+\<phi>reasoner_ML \<phi>Application 2000 (conclusion \<open>(PROP ?App) \<^bold>a\<^bold>p\<^bold>p\<^bold>l\<^bold>i\<^bold>e\<^bold>s ?State \<^bold>\<Rightarrow> (PROP ?Result)\<close>) =
   \<open>NuApply.start_reasoning\<close>
 
 \<phi>reasoner_ML \<phi>Application_Success 2000 (conclusion \<open>PROP \<phi>Application_Success\<close>) =
@@ -927,34 +934,54 @@ ML_file \<open>library/application.ML\<close>
 paragraph \<open>Common Rules of Application Methods\<close>
 
 lemma [\<phi>reason on \<open>
-  PROP \<phi>Application_Method (?App \<and> ?Apps) ?State ?Result
+  PROP \<phi>Application_Method (PROP ?App &&& PROP ?Apps) ?State ?Result
 \<close>]:
-  \<open> PROP \<phi>Application_Method  App State (PROP Result)
-\<Longrightarrow> PROP \<phi>Application_Method (App \<and> Apps) State (PROP Result)\<close>
-  unfolding prop_def \<phi>Application_def \<phi>Application_Method_def conj_imp .
+  \<open> PROP \<phi>Application_Method (PROP App) State (PROP Result)
+\<Longrightarrow> PROP \<phi>Application_Method (PROP App &&& PROP Apps) State (PROP Result)\<close>
+  unfolding prop_def \<phi>Application_def \<phi>Application_Method_def conjunction_imp .
 
 lemma [\<phi>reason on \<open>
-  PROP \<phi>Application_Method (?App \<and> ?Apps) ?State ?Result
+  PROP \<phi>Application_Method (PROP ?App &&& PROP ?Apps) ?State ?Result
 \<close>]:
-  \<open> PROP \<phi>Application_Method  Apps State (PROP Result)
-\<Longrightarrow> PROP \<phi>Application_Method (App \<and> Apps) State (PROP Result)\<close>
-  unfolding prop_def \<phi>Application_def \<phi>Application_Method_def conj_imp .
+  \<open> PROP \<phi>Application_Method (PROP Apps) State (PROP Result)
+\<Longrightarrow> PROP \<phi>Application_Method (PROP App &&& PROP Apps) State (PROP Result)\<close>
+  unfolding prop_def \<phi>Application_def \<phi>Application_Method_def conjunction_imp .
 
 lemma [\<phi>reason 1200 on \<open>
-  PROP \<phi>Application_Method (?Prem \<longrightarrow> ?App) ?State ?Result
+  PROP \<phi>Application_Method (PROP ?Prem \<Longrightarrow> PROP ?App) ?State ?Result
 \<close>]:
-  \<open> (Prem \<Longrightarrow> PROP \<phi>Application_Method  App State (PROP Result))
-\<Longrightarrow> PROP \<phi>Application_Method (Prem \<longrightarrow> App) State (Prem \<Longrightarrow> PROP Result)\<close>
+  \<open> (PROP Prem \<Longrightarrow> PROP \<phi>Application_Method (PROP App) State (PROP Result))
+\<Longrightarrow> PROP \<phi>Application_Method (PROP Prem \<Longrightarrow> PROP App) State (PROP Prem \<Longrightarrow> PROP Result)\<close>
   unfolding prop_def \<phi>Application_def \<phi>Application_Method_def imp_implication
-  subgoal premises prems using prems(1)[OF prems(4) prems(2) prems(3)[OF prems(4)]] . done
+  subgoal premises prems using prems(1)[OF prems(4) prems(2) prems(3)[OF prems(4)]] . .
 
 lemma [\<phi>reason 1200 on \<open>
-  PROP \<phi>Application_Method (All ?App) ?State ?Result
+  PROP \<phi>Application_Method (Trueprop (?Prem \<longrightarrow> ?App)) ?State ?Result
 \<close>]:
-  \<open> PROP \<phi>Application_Method (App x) State (PROP Result)
-\<Longrightarrow> PROP \<phi>Application_Method (All App) State (PROP Result)\<close>
+  \<open> (Prem \<Longrightarrow> PROP \<phi>Application_Method (Trueprop App) State (PROP Result))
+\<Longrightarrow> PROP \<phi>Application_Method (Trueprop (Prem \<longrightarrow> App)) State (Prem \<Longrightarrow> PROP Result)\<close>
   unfolding prop_def \<phi>Application_def \<phi>Application_Method_def imp_implication
-  subgoal premises prems using prems(1)[OF prems(2) prems(3)[THEN spec[where x=x]]] . done
+  subgoal premises prems using prems(1)[OF prems(4) prems(2) prems(3)[OF prems(4)]] . .
+
+
+lemma [\<phi>reason 1200 on \<open>
+  PROP \<phi>Application_Method (Pure.all ?App) ?State ?Result
+\<close>]:
+  \<open> PROP \<phi>Application_Method (PROP (App x)) State (PROP Result)
+\<Longrightarrow> PROP \<phi>Application_Method (Pure.all App) State (PROP Result)\<close>
+  unfolding \<phi>Application_def \<phi>Application_Method_def
+  subgoal premises prems
+    apply (tactic \<open>Tactic.resolve_tac \<^context>
+      [((Thm.forall_elim \<^cterm>\<open>x\<close> @{thm prems(3)}) RS @{thm prems(1)[OF prems(2)]})] 1\<close>) . .
+
+
+lemma [\<phi>reason 1200 on \<open>
+  PROP \<phi>Application_Method (Trueprop (All ?App)) ?State ?Result
+\<close>]:
+  \<open> PROP \<phi>Application_Method (Trueprop (App x)) State (PROP Result)
+\<Longrightarrow> PROP \<phi>Application_Method (Trueprop (All App)) State (PROP Result)\<close>
+  unfolding prop_def \<phi>Application_def \<phi>Application_Method_def imp_implication
+  subgoal premises prems using prems(1)[OF prems(2) prems(3)[THEN spec[where x=x]]] . .
 
 
 paragraph \<open>Application Methods\<close>
@@ -964,10 +991,11 @@ context std begin
 subparagraph \<open>Subtyping methods\<close>
 
 lemma \<phi>apply_subtyping_fast[\<phi>reason 2000 on \<open>
-  PROP \<phi>Application_Method (\<^bold>s\<^bold>u\<^bold>b\<^bold>t\<^bold>y\<^bold>p\<^bold>e ?S \<longmapsto> ?T \<^bold>w\<^bold>i\<^bold>t\<^bold>h ?P) (\<^bold>c\<^bold>u\<^bold>r\<^bold>r\<^bold>e\<^bold>n\<^bold>t ?blk [?RR] \<^bold>r\<^bold>e\<^bold>s\<^bold>u\<^bold>l\<^bold>t\<^bold>s \<^bold>i\<^bold>n ?S) ?Result
+  PROP \<phi>Application_Method (Trueprop (\<^bold>s\<^bold>u\<^bold>b\<^bold>t\<^bold>y\<^bold>p\<^bold>e ?S \<longmapsto> ?T \<^bold>w\<^bold>i\<^bold>t\<^bold>h ?P))
+          (\<^bold>c\<^bold>u\<^bold>r\<^bold>r\<^bold>e\<^bold>n\<^bold>t ?blk [?RR] \<^bold>r\<^bold>e\<^bold>s\<^bold>u\<^bold>l\<^bold>t\<^bold>s \<^bold>i\<^bold>n ?S) ?Result
 \<close>]:
   \<open> PROP \<phi>Application_Success
-\<Longrightarrow> PROP \<phi>Application_Method (\<^bold>s\<^bold>u\<^bold>b\<^bold>t\<^bold>y\<^bold>p\<^bold>e S \<longmapsto> T \<^bold>w\<^bold>i\<^bold>t\<^bold>h P)
+\<Longrightarrow> PROP \<phi>Application_Method (Trueprop (\<^bold>s\<^bold>u\<^bold>b\<^bold>t\<^bold>y\<^bold>p\<^bold>e S \<longmapsto> T \<^bold>w\<^bold>i\<^bold>t\<^bold>h P))
       (\<^bold>c\<^bold>u\<^bold>r\<^bold>r\<^bold>e\<^bold>n\<^bold>t blk [R] \<^bold>r\<^bold>e\<^bold>s\<^bold>u\<^bold>l\<^bold>t\<^bold>s \<^bold>i\<^bold>n S)
       (Trueprop ((\<^bold>c\<^bold>u\<^bold>r\<^bold>r\<^bold>e\<^bold>n\<^bold>t blk [R] \<^bold>r\<^bold>e\<^bold>s\<^bold>u\<^bold>l\<^bold>t\<^bold>s \<^bold>i\<^bold>n T) \<and> P))\<close>
   unfolding \<phi>Application_Method_def \<phi>Application_def
@@ -975,42 +1003,45 @@ lemma \<phi>apply_subtyping_fast[\<phi>reason 2000 on \<open>
 
 
 lemma \<phi>apply_subtyping_fully[\<phi>reason on \<open>
-  PROP \<phi>Application_Method (\<^bold>s\<^bold>u\<^bold>b\<^bold>t\<^bold>y\<^bold>p\<^bold>e ?S' \<longmapsto> ?T' \<^bold>w\<^bold>i\<^bold>t\<^bold>h ?P) (\<^bold>c\<^bold>u\<^bold>r\<^bold>r\<^bold>e\<^bold>n\<^bold>t ?blk [?RR] \<^bold>r\<^bold>e\<^bold>s\<^bold>u\<^bold>l\<^bold>t\<^bold>s \<^bold>i\<^bold>n ?S) ?Result
+  PROP \<phi>Application_Method (Trueprop (\<^bold>s\<^bold>u\<^bold>b\<^bold>t\<^bold>y\<^bold>p\<^bold>e ?S' \<longmapsto> ?T' \<^bold>w\<^bold>i\<^bold>t\<^bold>h ?P))
+      (\<^bold>c\<^bold>u\<^bold>r\<^bold>r\<^bold>e\<^bold>n\<^bold>t ?blk [?RR] \<^bold>r\<^bold>e\<^bold>s\<^bold>u\<^bold>l\<^bold>t\<^bold>s \<^bold>i\<^bold>n ?S) ?Result
 \<close>]:
   "IntroFrameVar R S'' S' T T'
 \<Longrightarrow> SUBGOAL TOP_GOAL G
-\<Longrightarrow> \<medium_left_bracket> \<^bold>s\<^bold>u\<^bold>b\<^bold>t\<^bold>y\<^bold>p\<^bold>e S \<longmapsto> \<medium_left_bracket> S'' \<medium_right_bracket> \<^bold>w\<^bold>i\<^bold>t\<^bold>h Any \<medium_right_bracket>: G
+\<Longrightarrow> \<^bold>s\<^bold>u\<^bold>b\<^bold>t\<^bold>y\<^bold>p\<^bold>e S \<longmapsto> \<blangle> S'' \<brangle> \<^bold>w\<^bold>i\<^bold>t\<^bold>h Any  \<^bold>@\<^bold>G\<^bold>O\<^bold>A\<^bold>L G
 \<Longrightarrow> SOLVE_SUBGOAL G
 \<Longrightarrow> PROP \<phi>Application_Success
 \<Longrightarrow> \<^bold>o\<^bold>b\<^bold>l\<^bold>i\<^bold>g\<^bold>a\<^bold>t\<^bold>i\<^bold>o\<^bold>n True
-\<Longrightarrow> PROP \<phi>Application_Method (\<^bold>s\<^bold>u\<^bold>b\<^bold>t\<^bold>y\<^bold>p\<^bold>e S' \<longmapsto> T' \<^bold>w\<^bold>i\<^bold>t\<^bold>h P)
+\<Longrightarrow> PROP \<phi>Application_Method (Trueprop (\<^bold>s\<^bold>u\<^bold>b\<^bold>t\<^bold>y\<^bold>p\<^bold>e S' \<longmapsto> T' \<^bold>w\<^bold>i\<^bold>t\<^bold>h P))
       (\<^bold>c\<^bold>u\<^bold>r\<^bold>r\<^bold>e\<^bold>n\<^bold>t blk [RR] \<^bold>r\<^bold>e\<^bold>s\<^bold>u\<^bold>l\<^bold>t\<^bold>s \<^bold>i\<^bold>n S)
       (Trueprop ((\<^bold>c\<^bold>u\<^bold>r\<^bold>r\<^bold>e\<^bold>n\<^bold>t blk [RR] \<^bold>r\<^bold>e\<^bold>s\<^bold>u\<^bold>l\<^bold>t\<^bold>s \<^bold>i\<^bold>n T) \<and> P))"
   unfolding IntroFrameVar_def \<phi>Application_Method_def \<phi>Application_def
-    Subty_Target2_def Subty_Target_def Subty_Target_def
+    GOAL_CTXT_def FOCUS_TAG_def
   using "\<phi>cast_P" \<phi>cast_intro_frame
   by (metis (no_types, lifting))
 
 
 lemma [\<phi>reason 2000 on \<open>
-  PROP \<phi>Application_Method (\<^bold>s\<^bold>u\<^bold>b\<^bold>t\<^bold>y\<^bold>p\<^bold>e ?S \<longmapsto> ?T \<^bold>w\<^bold>i\<^bold>t\<^bold>h ?P) (\<^bold>c\<^bold>u\<^bold>r\<^bold>r\<^bold>e\<^bold>n\<^bold>t ?blk [?RR] \<^bold>r\<^bold>e\<^bold>s\<^bold>u\<^bold>l\<^bold>t\<^bold>s \<^bold>i\<^bold>n VAL ?S) ?Result
+  PROP \<phi>Application_Method (Trueprop (\<^bold>s\<^bold>u\<^bold>b\<^bold>t\<^bold>y\<^bold>p\<^bold>e ?S \<longmapsto> ?T \<^bold>w\<^bold>i\<^bold>t\<^bold>h ?P))
+          (\<^bold>c\<^bold>u\<^bold>r\<^bold>r\<^bold>e\<^bold>n\<^bold>t ?blk [?RR] \<^bold>r\<^bold>e\<^bold>s\<^bold>u\<^bold>l\<^bold>t\<^bold>s \<^bold>i\<^bold>n VAL ?S) ?Result
 \<close>]:
   \<open> PROP \<phi>Application_Success
-\<Longrightarrow> PROP \<phi>Application_Method (\<^bold>s\<^bold>u\<^bold>b\<^bold>t\<^bold>y\<^bold>p\<^bold>e S \<longmapsto> T \<^bold>w\<^bold>i\<^bold>t\<^bold>h P)
+\<Longrightarrow> PROP \<phi>Application_Method (Trueprop (\<^bold>s\<^bold>u\<^bold>b\<^bold>t\<^bold>y\<^bold>p\<^bold>e S \<longmapsto> T \<^bold>w\<^bold>i\<^bold>t\<^bold>h P))
       (\<^bold>c\<^bold>u\<^bold>r\<^bold>r\<^bold>e\<^bold>n\<^bold>t blk [RR] \<^bold>r\<^bold>e\<^bold>s\<^bold>u\<^bold>l\<^bold>t\<^bold>s \<^bold>i\<^bold>n VAL S)
       (Trueprop ((\<^bold>c\<^bold>u\<^bold>r\<^bold>r\<^bold>e\<^bold>n\<^bold>t blk [RR] \<^bold>r\<^bold>e\<^bold>s\<^bold>u\<^bold>l\<^bold>t\<^bold>s \<^bold>i\<^bold>n VAL T) \<and> P))\<close>
   unfolding \<phi>Application_Method_def \<phi>Application_def
   using "\<phi>cast_P" cast_val_\<phi>app[unfolded Argument_def] by blast
 
 lemma [\<phi>reason 2000 on \<open>
-  PROP \<phi>Application_Method (\<^bold>s\<^bold>u\<^bold>b\<^bold>t\<^bold>y\<^bold>p\<^bold>e ?S' \<longmapsto> ?T \<^bold>w\<^bold>i\<^bold>t\<^bold>h ?P) (\<^bold>c\<^bold>u\<^bold>r\<^bold>r\<^bold>e\<^bold>n\<^bold>t ?blk [?RR] \<^bold>r\<^bold>e\<^bold>s\<^bold>u\<^bold>l\<^bold>t\<^bold>s \<^bold>i\<^bold>n VAL ?S) ?Result
+  PROP \<phi>Application_Method (Trueprop (\<^bold>s\<^bold>u\<^bold>b\<^bold>t\<^bold>y\<^bold>p\<^bold>e ?S' \<longmapsto> ?T \<^bold>w\<^bold>i\<^bold>t\<^bold>h ?P))
+      (\<^bold>c\<^bold>u\<^bold>r\<^bold>r\<^bold>e\<^bold>n\<^bold>t ?blk [?RR] \<^bold>r\<^bold>e\<^bold>s\<^bold>u\<^bold>l\<^bold>t\<^bold>s \<^bold>i\<^bold>n VAL ?S) ?Result
 \<close>]:
   \<open> SUBGOAL TOP_GOAL G
 \<Longrightarrow> \<^bold>s\<^bold>u\<^bold>b\<^bold>t\<^bold>y\<^bold>p\<^bold>e S \<longmapsto> S' \<^bold>w\<^bold>i\<^bold>t\<^bold>h Any
 \<Longrightarrow> SOLVE_SUBGOAL G
 \<Longrightarrow> PROP \<phi>Application_Success
 \<Longrightarrow> \<^bold>o\<^bold>b\<^bold>l\<^bold>i\<^bold>g\<^bold>a\<^bold>t\<^bold>i\<^bold>o\<^bold>n True
-\<Longrightarrow> PROP \<phi>Application_Method (\<^bold>s\<^bold>u\<^bold>b\<^bold>t\<^bold>y\<^bold>p\<^bold>e S' \<longmapsto> T \<^bold>w\<^bold>i\<^bold>t\<^bold>h P)
+\<Longrightarrow> PROP \<phi>Application_Method (Trueprop (\<^bold>s\<^bold>u\<^bold>b\<^bold>t\<^bold>y\<^bold>p\<^bold>e S' \<longmapsto> T \<^bold>w\<^bold>i\<^bold>t\<^bold>h P))
       (\<^bold>c\<^bold>u\<^bold>r\<^bold>r\<^bold>e\<^bold>n\<^bold>t blk [RR] \<^bold>r\<^bold>e\<^bold>s\<^bold>u\<^bold>l\<^bold>t\<^bold>s \<^bold>i\<^bold>n VAL S)
       (Trueprop ((\<^bold>c\<^bold>u\<^bold>r\<^bold>r\<^bold>e\<^bold>n\<^bold>t blk [RR] \<^bold>r\<^bold>e\<^bold>s\<^bold>u\<^bold>l\<^bold>t\<^bold>s \<^bold>i\<^bold>n VAL T) \<and> P))\<close>
   unfolding \<phi>Application_Method_def \<phi>Application_def
@@ -1018,24 +1049,26 @@ lemma [\<phi>reason 2000 on \<open>
 
 
 lemma [\<phi>reason 2000 on \<open>
-  PROP \<phi>Application_Method (\<^bold>s\<^bold>u\<^bold>b\<^bold>t\<^bold>y\<^bold>p\<^bold>e ?S \<longmapsto> ?T \<^bold>w\<^bold>i\<^bold>t\<^bold>h ?P) (\<^bold>c\<^bold>u\<^bold>r\<^bold>r\<^bold>e\<^bold>n\<^bold>t ?blk [?RR] \<^bold>r\<^bold>e\<^bold>s\<^bold>u\<^bold>l\<^bold>t\<^bold>s \<^bold>i\<^bold>n ?R\<heavy_comma> VAL ?S) ?Result
+  PROP \<phi>Application_Method (Trueprop (\<^bold>s\<^bold>u\<^bold>b\<^bold>t\<^bold>y\<^bold>p\<^bold>e ?S \<longmapsto> ?T \<^bold>w\<^bold>i\<^bold>t\<^bold>h ?P))
+          (\<^bold>c\<^bold>u\<^bold>r\<^bold>r\<^bold>e\<^bold>n\<^bold>t ?blk [?RR] \<^bold>r\<^bold>e\<^bold>s\<^bold>u\<^bold>l\<^bold>t\<^bold>s \<^bold>i\<^bold>n ?R\<heavy_comma> VAL ?S) ?Result
 \<close>]:
   \<open> PROP \<phi>Application_Success
-\<Longrightarrow> PROP \<phi>Application_Method (\<^bold>s\<^bold>u\<^bold>b\<^bold>t\<^bold>y\<^bold>p\<^bold>e S \<longmapsto> T \<^bold>w\<^bold>i\<^bold>t\<^bold>h P)
+\<Longrightarrow> PROP \<phi>Application_Method (Trueprop (\<^bold>s\<^bold>u\<^bold>b\<^bold>t\<^bold>y\<^bold>p\<^bold>e S \<longmapsto> T \<^bold>w\<^bold>i\<^bold>t\<^bold>h P))
       (\<^bold>c\<^bold>u\<^bold>r\<^bold>r\<^bold>e\<^bold>n\<^bold>t blk [RR] \<^bold>r\<^bold>e\<^bold>s\<^bold>u\<^bold>l\<^bold>t\<^bold>s \<^bold>i\<^bold>n R\<heavy_comma> VAL S)
       (Trueprop ((\<^bold>c\<^bold>u\<^bold>r\<^bold>r\<^bold>e\<^bold>n\<^bold>t blk [RR] \<^bold>r\<^bold>e\<^bold>s\<^bold>u\<^bold>l\<^bold>t\<^bold>s \<^bold>i\<^bold>n R\<heavy_comma> VAL T) \<and> P))\<close>
   unfolding \<phi>Application_Method_def \<phi>Application_def
   using "\<phi>cast_P" cast_val_\<phi>app[unfolded Argument_def] \<phi>cast_intro_frame by blast
 
 lemma [\<phi>reason 2000 on \<open>
-  PROP \<phi>Application_Method (\<^bold>s\<^bold>u\<^bold>b\<^bold>t\<^bold>y\<^bold>p\<^bold>e ?S' \<longmapsto> ?T \<^bold>w\<^bold>i\<^bold>t\<^bold>h ?P) (\<^bold>c\<^bold>u\<^bold>r\<^bold>r\<^bold>e\<^bold>n\<^bold>t ?blk [?RR] \<^bold>r\<^bold>e\<^bold>s\<^bold>u\<^bold>l\<^bold>t\<^bold>s \<^bold>i\<^bold>n ?R\<heavy_comma> VAL ?S) ?Result
+  PROP \<phi>Application_Method (Trueprop (\<^bold>s\<^bold>u\<^bold>b\<^bold>t\<^bold>y\<^bold>p\<^bold>e ?S' \<longmapsto> ?T \<^bold>w\<^bold>i\<^bold>t\<^bold>h ?P))
+          (\<^bold>c\<^bold>u\<^bold>r\<^bold>r\<^bold>e\<^bold>n\<^bold>t ?blk [?RR] \<^bold>r\<^bold>e\<^bold>s\<^bold>u\<^bold>l\<^bold>t\<^bold>s \<^bold>i\<^bold>n ?R\<heavy_comma> VAL ?S) ?Result
 \<close>]:
   \<open> SUBGOAL TOP_GOAL G
 \<Longrightarrow> \<^bold>s\<^bold>u\<^bold>b\<^bold>t\<^bold>y\<^bold>p\<^bold>e S \<longmapsto> S' \<^bold>w\<^bold>i\<^bold>t\<^bold>h Any
 \<Longrightarrow> SOLVE_SUBGOAL G
 \<Longrightarrow> PROP \<phi>Application_Success
 \<Longrightarrow> \<^bold>o\<^bold>b\<^bold>l\<^bold>i\<^bold>g\<^bold>a\<^bold>t\<^bold>i\<^bold>o\<^bold>n True
-\<Longrightarrow> PROP \<phi>Application_Method (\<^bold>s\<^bold>u\<^bold>b\<^bold>t\<^bold>y\<^bold>p\<^bold>e S' \<longmapsto> T \<^bold>w\<^bold>i\<^bold>t\<^bold>h P)
+\<Longrightarrow> PROP \<phi>Application_Method (Trueprop (\<^bold>s\<^bold>u\<^bold>b\<^bold>t\<^bold>y\<^bold>p\<^bold>e S' \<longmapsto> T \<^bold>w\<^bold>i\<^bold>t\<^bold>h P))
       (\<^bold>c\<^bold>u\<^bold>r\<^bold>r\<^bold>e\<^bold>n\<^bold>t blk [RR] \<^bold>r\<^bold>e\<^bold>s\<^bold>u\<^bold>l\<^bold>t\<^bold>s \<^bold>i\<^bold>n R\<heavy_comma> VAL S)
       (Trueprop ((\<^bold>c\<^bold>u\<^bold>r\<^bold>r\<^bold>e\<^bold>n\<^bold>t blk [RR] \<^bold>r\<^bold>e\<^bold>s\<^bold>u\<^bold>l\<^bold>t\<^bold>s \<^bold>i\<^bold>n R\<heavy_comma> VAL T) \<and> P))\<close>
   unfolding \<phi>Application_Method_def \<phi>Application_def
@@ -1046,10 +1079,11 @@ lemma [\<phi>reason 2000 on \<open>
 subparagraph \<open>Procedure methods\<close>
 
 lemma apply_proc_fast[\<phi>reason 2000 on \<open>
-  PROP \<phi>Application_Method (\<^bold>p\<^bold>r\<^bold>o\<^bold>c ?f \<lbrace> ?S \<longmapsto> ?T \<rbrace>) (\<^bold>c\<^bold>u\<^bold>r\<^bold>r\<^bold>e\<^bold>n\<^bold>t ?blk [?H] \<^bold>r\<^bold>e\<^bold>s\<^bold>u\<^bold>l\<^bold>t\<^bold>s \<^bold>i\<^bold>n ?S) ?Result
+  PROP \<phi>Application_Method (Trueprop (\<^bold>p\<^bold>r\<^bold>o\<^bold>c ?f \<lbrace> ?S \<longmapsto> ?T \<rbrace>))
+          (\<^bold>c\<^bold>u\<^bold>r\<^bold>r\<^bold>e\<^bold>n\<^bold>t ?blk [?H] \<^bold>r\<^bold>e\<^bold>s\<^bold>u\<^bold>l\<^bold>t\<^bold>s \<^bold>i\<^bold>n ?S) ?Result
 \<close>]:
   \<open> PROP \<phi>Application_Success
-\<Longrightarrow> PROP \<phi>Application_Method (\<^bold>p\<^bold>r\<^bold>o\<^bold>c f \<lbrace> S \<longmapsto> T \<rbrace>)
+\<Longrightarrow> PROP \<phi>Application_Method (Trueprop (\<^bold>p\<^bold>r\<^bold>o\<^bold>c f \<lbrace> S \<longmapsto> T \<rbrace>))
       (\<^bold>c\<^bold>u\<^bold>r\<^bold>r\<^bold>e\<^bold>n\<^bold>t blk [H] \<^bold>r\<^bold>e\<^bold>s\<^bold>u\<^bold>l\<^bold>t\<^bold>s \<^bold>i\<^bold>n S)
       (Trueprop (\<^bold>p\<^bold>e\<^bold>n\<^bold>d\<^bold>i\<^bold>n\<^bold>g f \<^bold>o\<^bold>n blk [H] \<^bold>r\<^bold>e\<^bold>s\<^bold>u\<^bold>l\<^bold>t\<^bold>s \<^bold>i\<^bold>n T))\<close>
   unfolding \<phi>Application_Method_def \<phi>Application_def
@@ -1057,19 +1091,20 @@ lemma apply_proc_fast[\<phi>reason 2000 on \<open>
 
 
 lemma \<phi>apply_proc_fully[\<phi>reason on
-    \<open>PROP \<phi>Application_Method (\<^bold>p\<^bold>r\<^bold>o\<^bold>c ?f \<lbrace> ?S' \<longmapsto> ?T' \<rbrace>) (\<^bold>c\<^bold>u\<^bold>r\<^bold>r\<^bold>e\<^bold>n\<^bold>t ?blk [?RR] \<^bold>r\<^bold>e\<^bold>s\<^bold>u\<^bold>l\<^bold>t\<^bold>s \<^bold>i\<^bold>n ?S) ?Result\<close>
+    \<open>PROP \<phi>Application_Method (Trueprop (\<^bold>p\<^bold>r\<^bold>o\<^bold>c ?f \<lbrace> ?S' \<longmapsto> ?T' \<rbrace>))
+            (\<^bold>c\<^bold>u\<^bold>r\<^bold>r\<^bold>e\<^bold>n\<^bold>t ?blk [?RR] \<^bold>r\<^bold>e\<^bold>s\<^bold>u\<^bold>l\<^bold>t\<^bold>s \<^bold>i\<^bold>n ?S) ?Result\<close>
 ]:
   \<open> IntroFrameVar R S'' S' T T'
 \<Longrightarrow> SUBGOAL TOP_GOAL G
-\<Longrightarrow> \<medium_left_bracket> \<^bold>s\<^bold>u\<^bold>b\<^bold>t\<^bold>y\<^bold>p\<^bold>e S \<longmapsto> \<medium_left_bracket> S'' \<medium_right_bracket> \<^bold>w\<^bold>i\<^bold>t\<^bold>h P \<medium_right_bracket>: G
+\<Longrightarrow> \<^bold>s\<^bold>u\<^bold>b\<^bold>t\<^bold>y\<^bold>p\<^bold>e S \<longmapsto> \<blangle> S'' \<brangle> \<^bold>w\<^bold>i\<^bold>t\<^bold>h P  \<^bold>@\<^bold>G\<^bold>O\<^bold>A\<^bold>L G
 \<Longrightarrow> SOLVE_SUBGOAL G
 \<Longrightarrow> PROP \<phi>Application_Success
 \<Longrightarrow> \<^bold>o\<^bold>b\<^bold>l\<^bold>i\<^bold>g\<^bold>a\<^bold>t\<^bold>i\<^bold>o\<^bold>n True
-\<Longrightarrow> PROP \<phi>Application_Method (\<^bold>p\<^bold>r\<^bold>o\<^bold>c f \<lbrace> S' \<longmapsto> T' \<rbrace>)
+\<Longrightarrow> PROP \<phi>Application_Method (Trueprop (\<^bold>p\<^bold>r\<^bold>o\<^bold>c f \<lbrace> S' \<longmapsto> T' \<rbrace>))
     (\<^bold>c\<^bold>u\<^bold>r\<^bold>r\<^bold>e\<^bold>n\<^bold>t blk [RR] \<^bold>r\<^bold>e\<^bold>s\<^bold>u\<^bold>l\<^bold>t\<^bold>s \<^bold>i\<^bold>n S)
     (Trueprop (\<^bold>p\<^bold>e\<^bold>n\<^bold>d\<^bold>i\<^bold>n\<^bold>g f \<^bold>o\<^bold>n blk [RR] \<^bold>r\<^bold>e\<^bold>s\<^bold>u\<^bold>l\<^bold>t\<^bold>s \<^bold>i\<^bold>n T))\<close>
   unfolding \<phi>Application_Method_def \<phi>Application_def IntroFrameVar_def
-    Subty_Target2_def Subty_Target_def
+    GOAL_CTXT_def FOCUS_TAG_def
   using "\<phi>cast" \<phi>apply_proc \<phi>frame[where R=R] by meson
 
 end
@@ -1525,20 +1560,20 @@ subsection \<open>General Tools\<close>
 
 lemma (in std) "_\<phi>cast_internal_rule_":
   " \<^bold>c\<^bold>u\<^bold>r\<^bold>r\<^bold>e\<^bold>n\<^bold>t blk [H] \<^bold>r\<^bold>e\<^bold>s\<^bold>u\<^bold>l\<^bold>t\<^bold>s \<^bold>i\<^bold>n T
-\<Longrightarrow> \<medium_left_bracket> \<^bold>s\<^bold>u\<^bold>b\<^bold>t\<^bold>y\<^bold>p\<^bold>e T \<longmapsto> \<medium_left_bracket> T' \<medium_right_bracket> \<^bold>w\<^bold>i\<^bold>t\<^bold>h Any \<medium_right_bracket>: TOP_GOAL
+\<Longrightarrow> \<^bold>s\<^bold>u\<^bold>b\<^bold>t\<^bold>y\<^bold>p\<^bold>e T \<longmapsto> \<blangle> T' \<brangle> \<^bold>w\<^bold>i\<^bold>t\<^bold>h Any  \<^bold>@\<^bold>G\<^bold>O\<^bold>A\<^bold>L TOP_GOAL
 \<Longrightarrow> \<r>Success
 \<Longrightarrow> \<^bold>o\<^bold>b\<^bold>l\<^bold>i\<^bold>g\<^bold>a\<^bold>t\<^bold>i\<^bold>o\<^bold>n True
 \<Longrightarrow> PROP Pure.prop (Trueprop (\<^bold>c\<^bold>u\<^bold>r\<^bold>r\<^bold>e\<^bold>n\<^bold>t blk [H] \<^bold>r\<^bold>e\<^bold>s\<^bold>u\<^bold>l\<^bold>t\<^bold>s \<^bold>i\<^bold>n T'))"
-  unfolding CurrentConstruction_def Subty_Target_def Subty_def Subty_Target2_def Pure.prop_def
+  unfolding CurrentConstruction_def GOAL_CTXT_def Subty_def FOCUS_TAG_def Pure.prop_def
   by (cases blk, simp_all add: pair_All \<phi>expns) blast
 
 lemma (in std) "_\<phi>cast_internal_rule_'":
   " \<^bold>p\<^bold>e\<^bold>n\<^bold>d\<^bold>i\<^bold>n\<^bold>g f \<^bold>o\<^bold>n blk [H] \<^bold>r\<^bold>e\<^bold>s\<^bold>u\<^bold>l\<^bold>t\<^bold>s \<^bold>i\<^bold>n T
-\<Longrightarrow> \<medium_left_bracket> \<^bold>s\<^bold>u\<^bold>b\<^bold>t\<^bold>y\<^bold>p\<^bold>e T \<longmapsto> \<medium_left_bracket> T' \<medium_right_bracket> \<^bold>w\<^bold>i\<^bold>t\<^bold>h Any \<medium_right_bracket>: TOP_GOAL
+\<Longrightarrow> \<^bold>s\<^bold>u\<^bold>b\<^bold>t\<^bold>y\<^bold>p\<^bold>e T \<longmapsto> \<blangle> T' \<brangle> \<^bold>w\<^bold>i\<^bold>t\<^bold>h Any  \<^bold>@\<^bold>G\<^bold>O\<^bold>A\<^bold>L TOP_GOAL
 \<Longrightarrow> \<r>Success
 \<Longrightarrow> \<^bold>o\<^bold>b\<^bold>l\<^bold>i\<^bold>g\<^bold>a\<^bold>t\<^bold>i\<^bold>o\<^bold>n True
 \<Longrightarrow> PROP Pure.prop(Trueprop (\<^bold>p\<^bold>e\<^bold>n\<^bold>d\<^bold>i\<^bold>n\<^bold>g f \<^bold>o\<^bold>n blk [H] \<^bold>r\<^bold>e\<^bold>s\<^bold>u\<^bold>l\<^bold>t\<^bold>s \<^bold>i\<^bold>n T'))"
-  unfolding Subty_Target_def Subty_def PendingConstruction_def bind_def Subty_Target2_def Pure.prop_def
+  unfolding FOCUS_TAG_def Subty_def PendingConstruction_def bind_def GOAL_CTXT_def Pure.prop_def
   by (cases blk, auto simp add: \<phi>expns LooseStateTy_expn') blast+
 
 
@@ -1609,163 +1644,169 @@ ML_file "library/reasoners.ML"
 
 subsection \<open>Subty Reasoning\<close>
 
-lemmas cast_def = Subty_Target_def Subty_Target2_def Subty_def
+lemmas cast_def = GOAL_CTXT_def FOCUS_TAG_def Subty_def
 
 (* lemma [\<phi>intro0]: "\<^bold>s\<^bold>u\<^bold>b\<^bold>t\<^bold>y\<^bold>p\<^bold>e x \<Ztypecolon> X \<longmapsto> H' * y \<Ztypecolon> Y \<^bold>w\<^bold>i\<^bold>t\<^bold>h P \<^bold>d\<^bold>u\<^bold>a\<^bold>l H'\<^sub>m * y\<^sub>m \<Ztypecolon> Y \<longmapsto> x\<^sub>m \<Ztypecolon> X \<^bold>w\<^bold>h\<^bold>e\<^bold>n Q
-  \<Longrightarrow> \<^bold>s\<^bold>u\<^bold>b\<^bold>t\<^bold>y\<^bold>p\<^bold>e x \<Ztypecolon> X \<longmapsto> H' * \<medium_left_bracket> y \<Ztypecolon> Y \<medium_right_bracket> \<^bold>w\<^bold>i\<^bold>t\<^bold>h P \<^bold>d\<^bold>u\<^bold>a\<^bold>l H'\<^sub>m * \<medium_left_bracket> y\<^sub>m \<Ztypecolon> Y \<medium_right_bracket> \<longmapsto> x\<^sub>m \<Ztypecolon> X \<^bold>w\<^bold>h\<^bold>e\<^bold>n Q"
+  \<Longrightarrow> \<^bold>s\<^bold>u\<^bold>b\<^bold>t\<^bold>y\<^bold>p\<^bold>e x \<Ztypecolon> X \<longmapsto> H' * \<blangle> y \<Ztypecolon> Y \<brangle> \<^bold>w\<^bold>i\<^bold>t\<^bold>h P \<^bold>d\<^bold>u\<^bold>a\<^bold>l H'\<^sub>m * \<blangle> y\<^sub>m \<Ztypecolon> Y \<brangle> \<longmapsto> x\<^sub>m \<Ztypecolon> X \<^bold>w\<^bold>h\<^bold>e\<^bold>n Q"
   unfolding Heap_Subty_Goal_def . *)
 (* lemma [\<phi>intro0]: "\<^bold>s\<^bold>u\<^bold>b\<^bold>t\<^bold>y\<^bold>p\<^bold>e A \<longmapsto> A \<^bold>d\<^bold>u\<^bold>a\<^bold>l B \<longmapsto> B" unfolding SubtyDual_def  by (simp add: cast_id) *)
 
 (* lemma [\<phi>intro 1000]:
-  "\<medium_left_bracket> \<^bold>s\<^bold>u\<^bold>b\<^bold>t\<^bold>y\<^bold>p\<^bold>e L * H \<longmapsto> L * H \<^bold>d\<^bold>u\<^bold>a\<^bold>l L * h\<^sub>m \<Ztypecolon> \<medium_left_bracket> H\<^sub>m \<medium_right_bracket> \<longmapsto> L * h\<^sub>m \<Ztypecolon> H\<^sub>m \<medium_right_bracket>"
+  "\<^bold>s\<^bold>u\<^bold>b\<^bold>t\<^bold>y\<^bold>p\<^bold>e L * H \<longmapsto> L * H \<^bold>d\<^bold>u\<^bold>a\<^bold>l L * h\<^sub>m \<Ztypecolon> \<blangle> H\<^sub>m \<brangle> \<longmapsto> L * h\<^sub>m \<Ztypecolon> H\<^sub>m \<brangle>"
   unfolding Heap_Subty_Goal_def using cast_dual_id . *)
 
 subsubsection \<open>Identity Subty\<close>
 
-lemma [\<phi>reason 3000 on \<open>\<medium_left_bracket> \<^bold>s\<^bold>u\<^bold>b\<^bold>t\<^bold>y\<^bold>p\<^bold>e ?H \<longmapsto> \<medium_left_bracket> ?H2 \<medium_right_bracket> \<^bold>w\<^bold>i\<^bold>t\<^bold>h ?P \<medium_right_bracket>: ?G\<close>]:
-      "\<medium_left_bracket> \<^bold>s\<^bold>u\<^bold>b\<^bold>t\<^bold>y\<^bold>p\<^bold>e H \<longmapsto> \<medium_left_bracket> H \<medium_right_bracket> \<medium_right_bracket>: G"
-  and [\<phi>reason 3000 on \<open>\<medium_left_bracket> \<^bold>s\<^bold>u\<^bold>b\<^bold>t\<^bold>y\<^bold>p\<^bold>e ?H \<longmapsto> ?R * \<medium_left_bracket> ?H2 \<medium_right_bracket> \<^bold>w\<^bold>i\<^bold>t\<^bold>h ?P \<medium_right_bracket>: ?G\<close>]:
-      "\<medium_left_bracket> \<^bold>s\<^bold>u\<^bold>b\<^bold>t\<^bold>y\<^bold>p\<^bold>e H \<longmapsto> 1 * \<medium_left_bracket> H \<medium_right_bracket> \<medium_right_bracket>: G"
+lemma [\<phi>reason 3000 on \<open>\<^bold>s\<^bold>u\<^bold>b\<^bold>t\<^bold>y\<^bold>p\<^bold>e ?H \<longmapsto> \<blangle> ?H2 \<brangle> \<^bold>w\<^bold>i\<^bold>t\<^bold>h ?P \<^bold>@\<^bold>G\<^bold>O\<^bold>A\<^bold>L ?G\<close>]:
+      "\<^bold>s\<^bold>u\<^bold>b\<^bold>t\<^bold>y\<^bold>p\<^bold>e H \<longmapsto> \<blangle> H \<brangle>  \<^bold>@\<^bold>G\<^bold>O\<^bold>A\<^bold>L G"
+  and [\<phi>reason 3000 on \<open>\<^bold>s\<^bold>u\<^bold>b\<^bold>t\<^bold>y\<^bold>p\<^bold>e ?H \<longmapsto> ?R * \<blangle> ?H2 \<brangle> \<^bold>w\<^bold>i\<^bold>t\<^bold>h ?P \<^bold>@\<^bold>G\<^bold>O\<^bold>A\<^bold>L ?G\<close>]:
+      "\<^bold>s\<^bold>u\<^bold>b\<^bold>t\<^bold>y\<^bold>p\<^bold>e H \<longmapsto> 1 * \<blangle> H \<brangle>  \<^bold>@\<^bold>G\<^bold>O\<^bold>A\<^bold>L G"
   for H :: \<open>'a::monoid_mult set\<close>
   unfolding cast_def mult_1_left by blast+
 
 (* lemma [\<phi>intro 40]: \<comment> \<open>outro\<close>
     "\<^bold>s\<^bold>i\<^bold>m\<^bold>p\<^bold>r\<^bold>e\<^bold>m a = a' \<Longrightarrow>
     \<^bold>s\<^bold>u\<^bold>b\<^bold>t\<^bold>y\<^bold>p\<^bold>e a \<Zinj> h \<Ztypecolon> H \<longmapsto> H' * a' \<Zinj> x \<Ztypecolon> X \<^bold>w\<^bold>i\<^bold>t\<^bold>h P \<^bold>d\<^bold>u\<^bold>a\<^bold>l H'\<^sub>m * a' \<Zinj> x\<^sub>m \<Ztypecolon> X\<^sub>m \<longmapsto> a \<Zinj> h\<^sub>m \<Ztypecolon> H\<^sub>m \<Longrightarrow>
-      \<medium_left_bracket> \<^bold>s\<^bold>u\<^bold>b\<^bold>t\<^bold>y\<^bold>p\<^bold>e a \<Zinj> h \<Ztypecolon> H \<longmapsto> H' * \<medium_left_bracket> Ele \<tort_lbrace> a' \<Zinj> x \<Ztypecolon> X \<tort_rbrace> \<medium_right_bracket> \<^bold>w\<^bold>i\<^bold>t\<^bold>h P \<^bold>d\<^bold>u\<^bold>a\<^bold>l H'\<^sub>m * \<medium_left_bracket> a' \<Zinj> x\<^sub>m \<Ztypecolon> X\<^sub>m \<medium_right_bracket> \<longmapsto> a \<Zinj> h\<^sub>m \<Ztypecolon> H\<^sub>m \<medium_right_bracket>"
+      \<^bold>s\<^bold>u\<^bold>b\<^bold>t\<^bold>y\<^bold>p\<^bold>e a \<Zinj> h \<Ztypecolon> H \<longmapsto> H' * \<blangle> Ele \<tort_lbrace> a' \<Zinj> x \<Ztypecolon> X \<tort_rbrace> \<brangle> \<^bold>w\<^bold>i\<^bold>t\<^bold>h P \<^bold>d\<^bold>u\<^bold>a\<^bold>l H'\<^sub>m * \<blangle> a' \<Zinj> x\<^sub>m \<Ztypecolon> X\<^sub>m \<brangle> \<longmapsto> a \<Zinj> h\<^sub>m \<Ztypecolon> H\<^sub>m \<brangle>"
   and [\<phi>intro 40]:
     "\<^bold>s\<^bold>i\<^bold>m\<^bold>p\<^bold>r\<^bold>e\<^bold>m a = a' \<Longrightarrow> 
-    \<^bold>s\<^bold>u\<^bold>b\<^bold>t\<^bold>y\<^bold>p\<^bold>e a \<Zinj> h \<Ztypecolon> H \<longmapsto> H' * a' \<Zinj> x \<Ztypecolon> X \<^bold>w\<^bold>i\<^bold>t\<^bold>h P \<Longrightarrow> \<medium_left_bracket> \<^bold>s\<^bold>u\<^bold>b\<^bold>t\<^bold>y\<^bold>p\<^bold>e a \<Zinj> h \<Ztypecolon> H \<longmapsto> H' * \<medium_left_bracket> a' \<Zinj> x \<Ztypecolon> X \<medium_right_bracket> \<^bold>w\<^bold>i\<^bold>t\<^bold>h P \<medium_right_bracket>"
+    \<^bold>s\<^bold>u\<^bold>b\<^bold>t\<^bold>y\<^bold>p\<^bold>e a \<Zinj> h \<Ztypecolon> H \<longmapsto> H' * a' \<Zinj> x \<Ztypecolon> X \<^bold>w\<^bold>i\<^bold>t\<^bold>h P \<Longrightarrow> \<^bold>s\<^bold>u\<^bold>b\<^bold>t\<^bold>y\<^bold>p\<^bold>e a \<Zinj> h \<Ztypecolon> H \<longmapsto> H' * \<blangle> a' \<Zinj> x \<Ztypecolon> X \<brangle> \<^bold>w\<^bold>i\<^bold>t\<^bold>h P \<brangle>"
   and [\<phi>intro 70]:
-    "\<^bold>s\<^bold>i\<^bold>m\<^bold>p\<^bold>r\<^bold>e\<^bold>m a = a' \<Longrightarrow> \<^bold>s\<^bold>u\<^bold>b\<^bold>t\<^bold>y\<^bold>p\<^bold>e a \<Zinj> h \<Ztypecolon> H \<longmapsto> a' \<Zinj> x \<Ztypecolon> X \<^bold>w\<^bold>i\<^bold>t\<^bold>h P \<Longrightarrow> \<medium_left_bracket> \<^bold>s\<^bold>u\<^bold>b\<^bold>t\<^bold>y\<^bold>p\<^bold>e a \<Zinj> h \<Ztypecolon> H \<longmapsto> 1 * \<medium_left_bracket> a' \<Zinj> x \<Ztypecolon> X \<medium_right_bracket> \<^bold>w\<^bold>i\<^bold>t\<^bold>h P \<medium_right_bracket>"*)
+    "\<^bold>s\<^bold>i\<^bold>m\<^bold>p\<^bold>r\<^bold>e\<^bold>m a = a' \<Longrightarrow> \<^bold>s\<^bold>u\<^bold>b\<^bold>t\<^bold>y\<^bold>p\<^bold>e a \<Zinj> h \<Ztypecolon> H \<longmapsto> a' \<Zinj> x \<Ztypecolon> X \<^bold>w\<^bold>i\<^bold>t\<^bold>h P \<Longrightarrow> \<^bold>s\<^bold>u\<^bold>b\<^bold>t\<^bold>y\<^bold>p\<^bold>e a \<Zinj> h \<Ztypecolon> H \<longmapsto> 1 * \<blangle> a' \<Zinj> x \<Ztypecolon> X \<brangle> \<^bold>w\<^bold>i\<^bold>t\<^bold>h P \<brangle>"*)
 (*  and [\<phi>intro 70]:
-    "\<^bold>s\<^bold>u\<^bold>b\<^bold>t\<^bold>y\<^bold>p\<^bold>e h \<Ztypecolon> H \<longmapsto> x \<Ztypecolon> X \<^bold>w\<^bold>i\<^bold>t\<^bold>h P \<Longrightarrow> \<medium_left_bracket> \<^bold>s\<^bold>u\<^bold>b\<^bold>t\<^bold>y\<^bold>p\<^bold>e h \<Ztypecolon> H \<longmapsto> \<medium_left_bracket> x \<Ztypecolon> X \<medium_right_bracket> \<^bold>w\<^bold>i\<^bold>t\<^bold>h P \<medium_right_bracket>" 
+    "\<^bold>s\<^bold>u\<^bold>b\<^bold>t\<^bold>y\<^bold>p\<^bold>e h \<Ztypecolon> H \<longmapsto> x \<Ztypecolon> X \<^bold>w\<^bold>i\<^bold>t\<^bold>h P \<Longrightarrow> \<^bold>s\<^bold>u\<^bold>b\<^bold>t\<^bold>y\<^bold>p\<^bold>e h \<Ztypecolon> H \<longmapsto> \<blangle> x \<Ztypecolon> X \<brangle> \<^bold>w\<^bold>i\<^bold>t\<^bold>h P \<brangle>" 
   unfolding Heap_Subty_Goal_def Separation_emptyL .*)
 
 context std begin
 
-subsubsection \<open>1 Holes\<close> \<comment> \<open>eliminate 1 holes generated during the reasoning \<close>
+subsubsection \<open>Void Holes\<close> \<comment> \<open>eliminate 1 holes generated during the reasoning \<close>
 
-lemma [\<phi>reason 2000]:
-  "\<medium_left_bracket> \<^bold>s\<^bold>u\<^bold>b\<^bold>t\<^bold>y\<^bold>p\<^bold>e H \<longmapsto> \<medium_left_bracket> X \<medium_right_bracket> \<^bold>w\<^bold>i\<^bold>t\<^bold>h P \<medium_right_bracket>: G \<Longrightarrow>
-   \<medium_left_bracket> \<^bold>s\<^bold>u\<^bold>b\<^bold>t\<^bold>y\<^bold>p\<^bold>e H \<longmapsto> \<medium_left_bracket> X \<heavy_comma> 1 \<medium_right_bracket> \<^bold>w\<^bold>i\<^bold>t\<^bold>h P \<medium_right_bracket>: G"
+lemma [\<phi>reason 2000 ]:
+  "\<^bold>s\<^bold>u\<^bold>b\<^bold>t\<^bold>y\<^bold>p\<^bold>e H \<longmapsto> \<blangle> X \<brangle> \<^bold>w\<^bold>i\<^bold>t\<^bold>h P \<^bold>@\<^bold>G\<^bold>O\<^bold>A\<^bold>L G \<Longrightarrow>
+   \<^bold>s\<^bold>u\<^bold>b\<^bold>t\<^bold>y\<^bold>p\<^bold>e H \<longmapsto> \<blangle> X \<heavy_comma> 1 \<brangle> \<^bold>w\<^bold>i\<^bold>t\<^bold>h P \<^bold>@\<^bold>G\<^bold>O\<^bold>A\<^bold>L G"
   unfolding cast_def mult_1_right .
 
-lemma [\<phi>reason 2000]:
-  "\<medium_left_bracket> \<^bold>s\<^bold>u\<^bold>b\<^bold>t\<^bold>y\<^bold>p\<^bold>e R \<longmapsto> X \<^bold>w\<^bold>i\<^bold>t\<^bold>h P \<medium_right_bracket>: G \<Longrightarrow>
-   \<medium_left_bracket> \<^bold>s\<^bold>u\<^bold>b\<^bold>t\<^bold>y\<^bold>p\<^bold>e R \<heavy_comma> 1 \<longmapsto> X \<^bold>w\<^bold>i\<^bold>t\<^bold>h P \<medium_right_bracket>: G"
+lemma [\<phi>reason 2000
+    if no \<open>\<^bold>s\<^bold>u\<^bold>b\<^bold>t\<^bold>y\<^bold>p\<^bold>e Void \<heavy_comma> Void \<longmapsto> ?X \<^bold>w\<^bold>i\<^bold>t\<^bold>h ?P \<^bold>@\<^bold>G\<^bold>O\<^bold>A\<^bold>L ?G\<close>
+]:
+  "\<^bold>s\<^bold>u\<^bold>b\<^bold>t\<^bold>y\<^bold>p\<^bold>e R \<longmapsto> X \<^bold>w\<^bold>i\<^bold>t\<^bold>h P \<^bold>@\<^bold>G\<^bold>O\<^bold>A\<^bold>L G \<Longrightarrow>
+   \<^bold>s\<^bold>u\<^bold>b\<^bold>t\<^bold>y\<^bold>p\<^bold>e R \<heavy_comma> Void \<longmapsto> X \<^bold>w\<^bold>i\<^bold>t\<^bold>h P \<^bold>@\<^bold>G\<^bold>O\<^bold>A\<^bold>L G"
   unfolding cast_def mult_1_right .
 
 subsubsection \<open>Pad 1 Holes at left\<close> \<comment> \<open>to standardize\<close>
 
-lemma [\<phi>reason 2000 if no \<open>\<medium_left_bracket> \<^bold>s\<^bold>u\<^bold>b\<^bold>t\<^bold>y\<^bold>p\<^bold>e ?H \<longmapsto> \<medium_left_bracket> (?X1 \<heavy_comma> ?X2) \<medium_right_bracket> \<^bold>w\<^bold>i\<^bold>t\<^bold>h ?P \<medium_right_bracket>: ?G\<close>]:
-  "\<medium_left_bracket> \<^bold>s\<^bold>u\<^bold>b\<^bold>t\<^bold>y\<^bold>p\<^bold>e H \<longmapsto> \<medium_left_bracket> 1 \<heavy_comma> X \<medium_right_bracket> \<^bold>w\<^bold>i\<^bold>t\<^bold>h P \<medium_right_bracket>: G \<Longrightarrow>
-   \<medium_left_bracket> \<^bold>s\<^bold>u\<^bold>b\<^bold>t\<^bold>y\<^bold>p\<^bold>e H \<longmapsto> \<medium_left_bracket> X \<medium_right_bracket> \<^bold>w\<^bold>i\<^bold>t\<^bold>h P \<medium_right_bracket>: G"
+lemma [\<phi>reason 2000
+  if no \<open>\<^bold>s\<^bold>u\<^bold>b\<^bold>t\<^bold>y\<^bold>p\<^bold>e ?H \<longmapsto> \<blangle> (?X1 \<heavy_comma> ?X2) \<brangle> \<^bold>w\<^bold>i\<^bold>t\<^bold>h ?P \<^bold>@\<^bold>G\<^bold>O\<^bold>A\<^bold>L ?G\<close>
+        \<open>\<^bold>s\<^bold>u\<^bold>b\<^bold>t\<^bold>y\<^bold>p\<^bold>e ?H \<longmapsto> \<blangle> Void \<brangle> \<^bold>w\<^bold>i\<^bold>t\<^bold>h ?P \<^bold>@\<^bold>G\<^bold>O\<^bold>A\<^bold>L ?G\<close>]:
+  "\<^bold>s\<^bold>u\<^bold>b\<^bold>t\<^bold>y\<^bold>p\<^bold>e H \<longmapsto> \<blangle> 1 \<heavy_comma> X \<brangle> \<^bold>w\<^bold>i\<^bold>t\<^bold>h P \<^bold>@\<^bold>G\<^bold>O\<^bold>A\<^bold>L G \<Longrightarrow>
+   \<^bold>s\<^bold>u\<^bold>b\<^bold>t\<^bold>y\<^bold>p\<^bold>e H \<longmapsto> \<blangle> X \<brangle> \<^bold>w\<^bold>i\<^bold>t\<^bold>h P \<^bold>@\<^bold>G\<^bold>O\<^bold>A\<^bold>L G"
   unfolding cast_def mult_1_left .
 
-lemma [\<phi>reason 2000 if no \<open>\<medium_left_bracket> \<^bold>s\<^bold>u\<^bold>b\<^bold>t\<^bold>y\<^bold>p\<^bold>e ?Y1 \<heavy_comma> ?Y2 \<longmapsto> ?X \<^bold>w\<^bold>i\<^bold>t\<^bold>h ?P \<medium_right_bracket>: ?G\<close>]:
-  "\<medium_left_bracket> \<^bold>s\<^bold>u\<^bold>b\<^bold>t\<^bold>y\<^bold>p\<^bold>e 1 \<heavy_comma> Y \<longmapsto> X \<^bold>w\<^bold>i\<^bold>t\<^bold>h P \<medium_right_bracket>: G \<Longrightarrow>
-   \<medium_left_bracket> \<^bold>s\<^bold>u\<^bold>b\<^bold>t\<^bold>y\<^bold>p\<^bold>e Y \<longmapsto> X \<^bold>w\<^bold>i\<^bold>t\<^bold>h P \<medium_right_bracket>: G"
+lemma [\<phi>reason 2000
+    if no \<open>\<^bold>s\<^bold>u\<^bold>b\<^bold>t\<^bold>y\<^bold>p\<^bold>e ?Y1 \<heavy_comma> ?Y2 \<longmapsto> ?X \<^bold>w\<^bold>i\<^bold>t\<^bold>h ?P \<^bold>@\<^bold>G\<^bold>O\<^bold>A\<^bold>L ?G\<close>
+]:
+  "\<^bold>s\<^bold>u\<^bold>b\<^bold>t\<^bold>y\<^bold>p\<^bold>e 1 \<heavy_comma> Y \<longmapsto> X \<^bold>w\<^bold>i\<^bold>t\<^bold>h P \<^bold>@\<^bold>G\<^bold>O\<^bold>A\<^bold>L G \<Longrightarrow>
+   \<^bold>s\<^bold>u\<^bold>b\<^bold>t\<^bold>y\<^bold>p\<^bold>e Y \<longmapsto> X \<^bold>w\<^bold>i\<^bold>t\<^bold>h P \<^bold>@\<^bold>G\<^bold>O\<^bold>A\<^bold>L G"
   unfolding cast_def mult_1_left .
 
 
 subsubsection \<open>Subjection\<close>
 
 lemma [\<phi>reason 2000]:
-  "\<medium_left_bracket> \<^bold>s\<^bold>u\<^bold>b\<^bold>t\<^bold>y\<^bold>p\<^bold>e T \<longmapsto> \<medium_left_bracket> U \<medium_right_bracket> \<^bold>w\<^bold>i\<^bold>t\<^bold>h P \<medium_right_bracket>: G \<Longrightarrow>
+  "\<^bold>s\<^bold>u\<^bold>b\<^bold>t\<^bold>y\<^bold>p\<^bold>e T \<longmapsto> \<blangle> U \<brangle> \<^bold>w\<^bold>i\<^bold>t\<^bold>h P \<^bold>@\<^bold>G\<^bold>O\<^bold>A\<^bold>L G \<Longrightarrow>
    (P \<Longrightarrow> \<^bold>p\<^bold>r\<^bold>e\<^bold>m\<^bold>i\<^bold>s\<^bold>e Q) \<Longrightarrow>
-   \<medium_left_bracket> \<^bold>s\<^bold>u\<^bold>b\<^bold>t\<^bold>y\<^bold>p\<^bold>e T \<longmapsto> \<medium_left_bracket> U \<^bold>s\<^bold>u\<^bold>b\<^bold>j Q \<medium_right_bracket> \<^bold>w\<^bold>i\<^bold>t\<^bold>h P \<medium_right_bracket>: G"
+   \<^bold>s\<^bold>u\<^bold>b\<^bold>t\<^bold>y\<^bold>p\<^bold>e T \<longmapsto> \<blangle> U \<^bold>s\<^bold>u\<^bold>b\<^bold>j Q \<brangle> \<^bold>w\<^bold>i\<^bold>t\<^bold>h P \<^bold>@\<^bold>G\<^bold>O\<^bold>A\<^bold>L G"
   unfolding cast_def by (simp add: \<phi>expns)
 
 lemma [\<phi>reason 2000]:
-  "\<medium_left_bracket> \<^bold>s\<^bold>u\<^bold>b\<^bold>t\<^bold>y\<^bold>p\<^bold>e T \<longmapsto> \<medium_left_bracket> R * U \<medium_right_bracket> \<^bold>w\<^bold>i\<^bold>t\<^bold>h P \<medium_right_bracket>: G \<Longrightarrow>
+  "\<^bold>s\<^bold>u\<^bold>b\<^bold>t\<^bold>y\<^bold>p\<^bold>e T \<longmapsto> \<blangle> R * U \<brangle> \<^bold>w\<^bold>i\<^bold>t\<^bold>h P \<^bold>@\<^bold>G\<^bold>O\<^bold>A\<^bold>L G \<Longrightarrow>
    (P \<Longrightarrow> \<^bold>p\<^bold>r\<^bold>e\<^bold>m\<^bold>i\<^bold>s\<^bold>e Q) \<Longrightarrow>
-   \<medium_left_bracket> \<^bold>s\<^bold>u\<^bold>b\<^bold>t\<^bold>y\<^bold>p\<^bold>e T \<longmapsto> \<medium_left_bracket> R * (U \<^bold>s\<^bold>u\<^bold>b\<^bold>j Q) \<medium_right_bracket> \<^bold>w\<^bold>i\<^bold>t\<^bold>h P \<medium_right_bracket>: G"
+   \<^bold>s\<^bold>u\<^bold>b\<^bold>t\<^bold>y\<^bold>p\<^bold>e T \<longmapsto> \<blangle> R * (U \<^bold>s\<^bold>u\<^bold>b\<^bold>j Q) \<brangle> \<^bold>w\<^bold>i\<^bold>t\<^bold>h P \<^bold>@\<^bold>G\<^bold>O\<^bold>A\<^bold>L G"
   unfolding cast_def by (simp add: \<phi>expns)
 
 lemma [\<phi>reason 2500]:
-  "(Q \<Longrightarrow> \<medium_left_bracket> \<^bold>s\<^bold>u\<^bold>b\<^bold>t\<^bold>y\<^bold>p\<^bold>e T \<longmapsto> U \<^bold>w\<^bold>i\<^bold>t\<^bold>h P \<medium_right_bracket>: G) \<Longrightarrow>
-   \<medium_left_bracket> \<^bold>s\<^bold>u\<^bold>b\<^bold>t\<^bold>y\<^bold>p\<^bold>e T \<^bold>s\<^bold>u\<^bold>b\<^bold>j Q \<longmapsto> U \<^bold>w\<^bold>i\<^bold>t\<^bold>h P \<medium_right_bracket>: G"
+  "(Q \<Longrightarrow> \<^bold>s\<^bold>u\<^bold>b\<^bold>t\<^bold>y\<^bold>p\<^bold>e T \<longmapsto> U \<^bold>w\<^bold>i\<^bold>t\<^bold>h P \<^bold>@\<^bold>G\<^bold>O\<^bold>A\<^bold>L G) \<Longrightarrow>
+   \<^bold>s\<^bold>u\<^bold>b\<^bold>t\<^bold>y\<^bold>p\<^bold>e T \<^bold>s\<^bold>u\<^bold>b\<^bold>j Q \<longmapsto> U \<^bold>w\<^bold>i\<^bold>t\<^bold>h P \<^bold>@\<^bold>G\<^bold>O\<^bold>A\<^bold>L G"
   unfolding cast_def by (simp add: \<phi>expns) blast
 
 
 subsubsection \<open>Protector\<close>
 
 lemma [\<phi>reason 2000]:
-  "\<medium_left_bracket> \<^bold>s\<^bold>u\<^bold>b\<^bold>t\<^bold>y\<^bold>p\<^bold>e T \<longmapsto> \<medium_left_bracket> U \<medium_right_bracket> \<^bold>w\<^bold>i\<^bold>t\<^bold>h P \<medium_right_bracket>: G \<Longrightarrow>
-   \<medium_left_bracket> \<^bold>s\<^bold>u\<^bold>b\<^bold>t\<^bold>y\<^bold>p\<^bold>e T \<longmapsto> \<medium_left_bracket> \<^bold>( U \<^bold>) \<medium_right_bracket> \<^bold>w\<^bold>i\<^bold>t\<^bold>h P \<medium_right_bracket>: G"
+  "\<^bold>s\<^bold>u\<^bold>b\<^bold>t\<^bold>y\<^bold>p\<^bold>e T \<longmapsto> \<blangle> U \<brangle> \<^bold>w\<^bold>i\<^bold>t\<^bold>h P \<^bold>@\<^bold>G\<^bold>O\<^bold>A\<^bold>L G \<Longrightarrow>
+   \<^bold>s\<^bold>u\<^bold>b\<^bold>t\<^bold>y\<^bold>p\<^bold>e T \<longmapsto> \<blangle> \<^bold>( U \<^bold>) \<brangle> \<^bold>w\<^bold>i\<^bold>t\<^bold>h P \<^bold>@\<^bold>G\<^bold>O\<^bold>A\<^bold>L G"
   unfolding cast_def Implicit_Protector_def by (simp add: \<phi>expns)
 
 
 subsubsection \<open>Existential\<close>
 
 lemma [\<phi>reason 2000]:
-  "\<medium_left_bracket> \<^bold>s\<^bold>u\<^bold>b\<^bold>t\<^bold>y\<^bold>p\<^bold>e T \<longmapsto> \<medium_left_bracket> U c \<medium_right_bracket> \<^bold>w\<^bold>i\<^bold>t\<^bold>h P \<medium_right_bracket>: G \<Longrightarrow>
-   \<medium_left_bracket> \<^bold>s\<^bold>u\<^bold>b\<^bold>t\<^bold>y\<^bold>p\<^bold>e T \<longmapsto> \<medium_left_bracket> ExSet U \<medium_right_bracket> \<^bold>w\<^bold>i\<^bold>t\<^bold>h P \<medium_right_bracket>: G"
+  "\<^bold>s\<^bold>u\<^bold>b\<^bold>t\<^bold>y\<^bold>p\<^bold>e T \<longmapsto> \<blangle> U c \<brangle> \<^bold>w\<^bold>i\<^bold>t\<^bold>h P \<^bold>@\<^bold>G\<^bold>O\<^bold>A\<^bold>L G \<Longrightarrow>
+   \<^bold>s\<^bold>u\<^bold>b\<^bold>t\<^bold>y\<^bold>p\<^bold>e T \<longmapsto> \<blangle> ExSet U \<brangle> \<^bold>w\<^bold>i\<^bold>t\<^bold>h P \<^bold>@\<^bold>G\<^bold>O\<^bold>A\<^bold>L G"
   unfolding cast_def by (simp add: \<phi>expns) blast
 
 lemma [\<phi>reason 2500]:
-  "(\<And>x. \<medium_left_bracket> \<^bold>s\<^bold>u\<^bold>b\<^bold>t\<^bold>y\<^bold>p\<^bold>e T x \<longmapsto> U \<^bold>w\<^bold>i\<^bold>t\<^bold>h P \<medium_right_bracket>: G) \<Longrightarrow>
-   \<medium_left_bracket> \<^bold>s\<^bold>u\<^bold>b\<^bold>t\<^bold>y\<^bold>p\<^bold>e ExSet T \<longmapsto> U \<^bold>w\<^bold>i\<^bold>t\<^bold>h P \<medium_right_bracket>: G"
+  "(\<And>x. \<^bold>s\<^bold>u\<^bold>b\<^bold>t\<^bold>y\<^bold>p\<^bold>e T x \<longmapsto> U \<^bold>w\<^bold>i\<^bold>t\<^bold>h P \<^bold>@\<^bold>G\<^bold>O\<^bold>A\<^bold>L G) \<Longrightarrow>
+   \<^bold>s\<^bold>u\<^bold>b\<^bold>t\<^bold>y\<^bold>p\<^bold>e ExSet T \<longmapsto> U \<^bold>w\<^bold>i\<^bold>t\<^bold>h P \<^bold>@\<^bold>G\<^bold>O\<^bold>A\<^bold>L G"
   unfolding cast_def by (simp add: \<phi>expns) blast
 
 (* subsubsection \<open>Tailling\<close> \<comment> \<open>\<close>
 
 lemma [\<phi>intro 1100]: \<comment> \<open>tail the step\<close>
-  "\<medium_left_bracket> \<^bold>s\<^bold>u\<^bold>b\<^bold>t\<^bold>y\<^bold>p\<^bold>e H \<longmapsto> 1 \<heavy_comma> \<medium_left_bracket> x \<Ztypecolon> X \<medium_right_bracket> \<^bold>w\<^bold>i\<^bold>t\<^bold>h P \<^bold>d\<^bold>u\<^bold>a\<^bold>l 1 \<heavy_comma> \<medium_left_bracket> x\<^sub>m \<Ztypecolon> X\<^sub>m \<medium_right_bracket> \<longmapsto> H\<^sub>m \<medium_right_bracket> \<Longrightarrow>
-  \<medium_left_bracket> \<^bold>s\<^bold>u\<^bold>b\<^bold>t\<^bold>y\<^bold>p\<^bold>e H \<longmapsto> \<medium_left_bracket> VAL x \<Ztypecolon> X \<medium_right_bracket> \<^bold>w\<^bold>i\<^bold>t\<^bold>h P \<^bold>d\<^bold>u\<^bold>a\<^bold>l H\<^sub>m \<longmapsto> H\<^sub>m \<medium_right_bracket> "
+  "\<^bold>s\<^bold>u\<^bold>b\<^bold>t\<^bold>y\<^bold>p\<^bold>e H \<longmapsto> 1 \<heavy_comma> \<blangle> x \<Ztypecolon> X \<brangle> \<^bold>w\<^bold>i\<^bold>t\<^bold>h P \<^bold>d\<^bold>u\<^bold>a\<^bold>l 1 \<heavy_comma> \<blangle> x\<^sub>m \<Ztypecolon> X\<^sub>m \<brangle> \<longmapsto> H\<^sub>m \<brangle> \<Longrightarrow>
+  \<^bold>s\<^bold>u\<^bold>b\<^bold>t\<^bold>y\<^bold>p\<^bold>e H \<longmapsto> \<blangle> VAL x \<Ztypecolon> X \<brangle> \<^bold>w\<^bold>i\<^bold>t\<^bold>h P \<^bold>d\<^bold>u\<^bold>a\<^bold>l H\<^sub>m \<longmapsto> H\<^sub>m \<brangle> "
   unfolding Separation_emptyL Separation_emptyR .
 
 lemma [\<phi>intro 1100]: \<comment> \<open>tail the step\<close>
-  "\<medium_left_bracket> \<^bold>s\<^bold>u\<^bold>b\<^bold>t\<^bold>y\<^bold>p\<^bold>e H \<longmapsto> 1 \<heavy_comma> \<medium_left_bracket> x \<Ztypecolon> X \<medium_right_bracket> \<^bold>w\<^bold>i\<^bold>t\<^bold>h P \<^bold>d\<^bold>u\<^bold>a\<^bold>l 1 \<heavy_comma> \<medium_left_bracket> x\<^sub>m \<Ztypecolon> X\<^sub>m \<medium_right_bracket> \<longmapsto> H\<^sub>m \<medium_right_bracket> \<Longrightarrow>
-  \<medium_left_bracket> \<^bold>s\<^bold>u\<^bold>b\<^bold>t\<^bold>y\<^bold>p\<^bold>e H \<longmapsto> \<medium_left_bracket> x \<Ztypecolon> X \<medium_right_bracket> \<^bold>w\<^bold>i\<^bold>t\<^bold>h P \<^bold>d\<^bold>u\<^bold>a\<^bold>l \<medium_left_bracket> x\<^sub>m \<Ztypecolon> X\<^sub>m \<medium_right_bracket> \<longmapsto> H\<^sub>m \<medium_right_bracket> "
+  "\<^bold>s\<^bold>u\<^bold>b\<^bold>t\<^bold>y\<^bold>p\<^bold>e H \<longmapsto> 1 \<heavy_comma> \<blangle> x \<Ztypecolon> X \<brangle> \<^bold>w\<^bold>i\<^bold>t\<^bold>h P \<^bold>d\<^bold>u\<^bold>a\<^bold>l 1 \<heavy_comma> \<blangle> x\<^sub>m \<Ztypecolon> X\<^sub>m \<brangle> \<longmapsto> H\<^sub>m \<brangle> \<Longrightarrow>
+  \<^bold>s\<^bold>u\<^bold>b\<^bold>t\<^bold>y\<^bold>p\<^bold>e H \<longmapsto> \<blangle> x \<Ztypecolon> X \<brangle> \<^bold>w\<^bold>i\<^bold>t\<^bold>h P \<^bold>d\<^bold>u\<^bold>a\<^bold>l \<blangle> x\<^sub>m \<Ztypecolon> X\<^sub>m \<brangle> \<longmapsto> H\<^sub>m \<brangle> "
   unfolding Separation_emptyL Separation_emptyR .
 *)
 
 subsubsection \<open>Value\<close>
 
 
-lemma [\<phi>reason 2000 on \<open>\<medium_left_bracket> \<^bold>s\<^bold>u\<^bold>b\<^bold>t\<^bold>y\<^bold>p\<^bold>e ?R \<heavy_comma> (OBJ ?H) \<longmapsto> ?R''' \<heavy_comma> \<medium_left_bracket> VAL ?X \<medium_right_bracket> \<^bold>w\<^bold>i\<^bold>t\<^bold>h ?P \<medium_right_bracket>: ?G\<close>]:
-  " \<medium_left_bracket> \<^bold>s\<^bold>u\<^bold>b\<^bold>t\<^bold>y\<^bold>p\<^bold>e R \<longmapsto> R' \<heavy_comma> \<medium_left_bracket> VAL X \<medium_right_bracket> \<^bold>w\<^bold>i\<^bold>t\<^bold>h P \<medium_right_bracket>: G
-\<Longrightarrow> \<medium_left_bracket> \<^bold>s\<^bold>u\<^bold>b\<^bold>t\<^bold>y\<^bold>p\<^bold>e R \<heavy_comma> (OBJ H) \<longmapsto> R' \<heavy_comma> (OBJ H) \<heavy_comma> \<medium_left_bracket> VAL X \<medium_right_bracket> \<^bold>w\<^bold>i\<^bold>t\<^bold>h P \<medium_right_bracket>: G "
+lemma [\<phi>reason 2000 on \<open>\<^bold>s\<^bold>u\<^bold>b\<^bold>t\<^bold>y\<^bold>p\<^bold>e ?R \<heavy_comma> (OBJ ?H) \<longmapsto> ?R''' \<heavy_comma> \<blangle> VAL ?X \<brangle> \<^bold>w\<^bold>i\<^bold>t\<^bold>h ?P \<^bold>@\<^bold>G\<^bold>O\<^bold>A\<^bold>L ?G\<close>]:
+  " \<^bold>s\<^bold>u\<^bold>b\<^bold>t\<^bold>y\<^bold>p\<^bold>e R \<longmapsto> R' \<heavy_comma> \<blangle> VAL X \<brangle> \<^bold>w\<^bold>i\<^bold>t\<^bold>h P \<^bold>@\<^bold>G\<^bold>O\<^bold>A\<^bold>L G
+\<Longrightarrow> \<^bold>s\<^bold>u\<^bold>b\<^bold>t\<^bold>y\<^bold>p\<^bold>e R \<heavy_comma> (OBJ H) \<longmapsto> R' \<heavy_comma> (OBJ H) \<heavy_comma> \<blangle> VAL X \<brangle> \<^bold>w\<^bold>i\<^bold>t\<^bold>h P \<^bold>@\<^bold>G\<^bold>O\<^bold>A\<^bold>L G "
   unfolding cast_def pair_forall
   by (simp add: \<phi>expns times_list_def) metis
 
-lemma [\<phi>reason 2000 on \<open>\<medium_left_bracket> \<^bold>s\<^bold>u\<^bold>b\<^bold>t\<^bold>y\<^bold>p\<^bold>e ?R \<heavy_comma> (VAL ?V) \<longmapsto> ?R''' \<heavy_comma> \<medium_left_bracket> VAL ?X \<medium_right_bracket> \<^bold>w\<^bold>i\<^bold>t\<^bold>h ?P \<medium_right_bracket>: ?G\<close>]:
+lemma [\<phi>reason 2000 on \<open>\<^bold>s\<^bold>u\<^bold>b\<^bold>t\<^bold>y\<^bold>p\<^bold>e ?R \<heavy_comma> (VAL ?V) \<longmapsto> ?R''' \<heavy_comma> \<blangle> VAL ?X \<brangle> \<^bold>w\<^bold>i\<^bold>t\<^bold>h ?P \<^bold>@\<^bold>G\<^bold>O\<^bold>A\<^bold>L ?G\<close>]:
   " \<^bold>s\<^bold>u\<^bold>b\<^bold>t\<^bold>y\<^bold>p\<^bold>e V \<longmapsto> X \<^bold>w\<^bold>i\<^bold>t\<^bold>h P
-\<Longrightarrow> \<medium_left_bracket> \<^bold>s\<^bold>u\<^bold>b\<^bold>t\<^bold>y\<^bold>p\<^bold>e R \<heavy_comma> (VAL V) \<longmapsto> R \<heavy_comma> \<medium_left_bracket> VAL X \<medium_right_bracket> \<^bold>w\<^bold>i\<^bold>t\<^bold>h P \<medium_right_bracket>: G"
+\<Longrightarrow> \<^bold>s\<^bold>u\<^bold>b\<^bold>t\<^bold>y\<^bold>p\<^bold>e R \<heavy_comma> (VAL V) \<longmapsto> R \<heavy_comma> \<blangle> VAL X \<brangle> \<^bold>w\<^bold>i\<^bold>t\<^bold>h P \<^bold>@\<^bold>G\<^bold>O\<^bold>A\<^bold>L G"
   unfolding cast_def pair_forall
   by (simp add: \<phi>expns times_list_def) metis
 
-lemma [\<phi>reason 2000 on \<open>\<medium_left_bracket> \<^bold>s\<^bold>u\<^bold>b\<^bold>t\<^bold>y\<^bold>p\<^bold>e ?R \<longmapsto> \<medium_left_bracket> ?R2 \<heavy_comma> (VAL ?X) \<medium_right_bracket> \<^bold>w\<^bold>i\<^bold>t\<^bold>h ?P \<medium_right_bracket>: ?G\<close>]:
-  " \<medium_left_bracket> \<^bold>s\<^bold>u\<^bold>b\<^bold>t\<^bold>y\<^bold>p\<^bold>e R \<longmapsto> R1 \<heavy_comma> \<medium_left_bracket> VAL X \<medium_right_bracket> \<^bold>w\<^bold>i\<^bold>t\<^bold>h P1 \<medium_right_bracket>: G
-\<Longrightarrow> \<medium_left_bracket> \<^bold>s\<^bold>u\<^bold>b\<^bold>t\<^bold>y\<^bold>p\<^bold>e R1 \<longmapsto> \<medium_left_bracket> R2 \<medium_right_bracket> \<^bold>w\<^bold>i\<^bold>t\<^bold>h P2  \<medium_right_bracket>: G
-\<Longrightarrow> \<medium_left_bracket> \<^bold>s\<^bold>u\<^bold>b\<^bold>t\<^bold>y\<^bold>p\<^bold>e R \<longmapsto> \<medium_left_bracket> R2 \<heavy_comma> (VAL X) \<medium_right_bracket> \<^bold>w\<^bold>i\<^bold>t\<^bold>h P1 \<and> P2 \<medium_right_bracket>: G"
+lemma [\<phi>reason 2000 on \<open>\<^bold>s\<^bold>u\<^bold>b\<^bold>t\<^bold>y\<^bold>p\<^bold>e ?R \<longmapsto> \<blangle> ?R2 \<heavy_comma> (VAL ?X) \<brangle> \<^bold>w\<^bold>i\<^bold>t\<^bold>h ?P \<^bold>@\<^bold>G\<^bold>O\<^bold>A\<^bold>L ?G\<close>]:
+  " \<^bold>s\<^bold>u\<^bold>b\<^bold>t\<^bold>y\<^bold>p\<^bold>e R \<longmapsto> R1 \<heavy_comma> \<blangle> VAL X \<brangle> \<^bold>w\<^bold>i\<^bold>t\<^bold>h P1 \<^bold>@\<^bold>G\<^bold>O\<^bold>A\<^bold>L G
+\<Longrightarrow> \<^bold>s\<^bold>u\<^bold>b\<^bold>t\<^bold>y\<^bold>p\<^bold>e R1 \<longmapsto> \<blangle> R2 \<brangle> \<^bold>w\<^bold>i\<^bold>t\<^bold>h P2  \<^bold>@\<^bold>G\<^bold>O\<^bold>A\<^bold>L G
+\<Longrightarrow> \<^bold>s\<^bold>u\<^bold>b\<^bold>t\<^bold>y\<^bold>p\<^bold>e R \<longmapsto> \<blangle> R2 \<heavy_comma> (VAL X) \<brangle> \<^bold>w\<^bold>i\<^bold>t\<^bold>h P1 \<and> P2 \<^bold>@\<^bold>G\<^bold>O\<^bold>A\<^bold>L G"
   unfolding cast_def pair_forall
   by (simp add: \<phi>expns) metis
 
-lemma [\<phi>reason 2000 on \<open>\<medium_left_bracket> \<^bold>s\<^bold>u\<^bold>b\<^bold>t\<^bold>y\<^bold>p\<^bold>e ?R \<longmapsto> \<medium_left_bracket> ?R2 \<heavy_comma> (VAL ?X) \<medium_right_bracket> \<^bold>w\<^bold>i\<^bold>t\<^bold>h ?P \<medium_right_bracket>: ?G\<close>]:
-  " \<medium_left_bracket> \<^bold>s\<^bold>u\<^bold>b\<^bold>t\<^bold>y\<^bold>p\<^bold>e R \<longmapsto> R1 \<heavy_comma> \<medium_left_bracket> VAL X \<medium_right_bracket> \<^bold>w\<^bold>i\<^bold>t\<^bold>h P1 \<medium_right_bracket>: G
-\<Longrightarrow> \<medium_left_bracket> \<^bold>s\<^bold>u\<^bold>b\<^bold>t\<^bold>y\<^bold>p\<^bold>e R1 \<longmapsto> \<medium_left_bracket> R2 \<medium_right_bracket> \<^bold>w\<^bold>i\<^bold>t\<^bold>h P2  \<medium_right_bracket>: G
-\<Longrightarrow> \<medium_left_bracket> \<^bold>s\<^bold>u\<^bold>b\<^bold>t\<^bold>y\<^bold>p\<^bold>e R \<longmapsto> \<medium_left_bracket> R2 \<heavy_comma> (VAL X) \<medium_right_bracket> \<^bold>w\<^bold>i\<^bold>t\<^bold>h P1 \<and> P2 \<medium_right_bracket>: G"
+lemma [\<phi>reason 2000 on \<open>\<^bold>s\<^bold>u\<^bold>b\<^bold>t\<^bold>y\<^bold>p\<^bold>e ?R \<longmapsto> \<blangle> ?R2 \<heavy_comma> (VAL ?X) \<brangle> \<^bold>w\<^bold>i\<^bold>t\<^bold>h ?P \<^bold>@\<^bold>G\<^bold>O\<^bold>A\<^bold>L ?G\<close>]:
+  " \<^bold>s\<^bold>u\<^bold>b\<^bold>t\<^bold>y\<^bold>p\<^bold>e R \<longmapsto> R1 \<heavy_comma> \<blangle> VAL X \<brangle> \<^bold>w\<^bold>i\<^bold>t\<^bold>h P1 \<^bold>@\<^bold>G\<^bold>O\<^bold>A\<^bold>L G
+\<Longrightarrow> \<^bold>s\<^bold>u\<^bold>b\<^bold>t\<^bold>y\<^bold>p\<^bold>e R1 \<longmapsto> \<blangle> R2 \<brangle> \<^bold>w\<^bold>i\<^bold>t\<^bold>h P2  \<^bold>@\<^bold>G\<^bold>O\<^bold>A\<^bold>L G
+\<Longrightarrow> \<^bold>s\<^bold>u\<^bold>b\<^bold>t\<^bold>y\<^bold>p\<^bold>e R \<longmapsto> \<blangle> R2 \<heavy_comma> (VAL X) \<brangle> \<^bold>w\<^bold>i\<^bold>t\<^bold>h P1 \<and> P2 \<^bold>@\<^bold>G\<^bold>O\<^bold>A\<^bold>L G"
   unfolding cast_def pair_forall
   by (simp add: \<phi>expns) metis
 
 
 subsubsection \<open>Object\<close>
 
-lemma [\<phi>reason 100 on \<open>\<medium_left_bracket> \<^bold>s\<^bold>u\<^bold>b\<^bold>t\<^bold>y\<^bold>p\<^bold>e ?R \<heavy_comma> OBJ ?H \<longmapsto> ?R''' * \<medium_left_bracket> OBJ ?X \<medium_right_bracket> \<^bold>w\<^bold>i\<^bold>t\<^bold>h ?P \<medium_right_bracket>: ?G\<close>]: \<comment> \<open>attempts the immediate cell\<close>
+lemma [\<phi>reason 100 on \<open>\<^bold>s\<^bold>u\<^bold>b\<^bold>t\<^bold>y\<^bold>p\<^bold>e ?R \<heavy_comma> OBJ ?H \<longmapsto> ?R''' * \<blangle> OBJ ?X \<brangle> \<^bold>w\<^bold>i\<^bold>t\<^bold>h ?P \<^bold>@\<^bold>G\<^bold>O\<^bold>A\<^bold>L ?G\<close>]: \<comment> \<open>attempts the immediate cell\<close>
   " CHK_SUBGOAL G
   \<Longrightarrow> \<^bold>s\<^bold>u\<^bold>b\<^bold>t\<^bold>y\<^bold>p\<^bold>e OBJ H \<longmapsto> H'\<heavy_comma> OBJ X \<^bold>w\<^bold>i\<^bold>t\<^bold>h P
-  \<Longrightarrow> \<medium_left_bracket> \<^bold>s\<^bold>u\<^bold>b\<^bold>t\<^bold>y\<^bold>p\<^bold>e R\<heavy_comma> OBJ H \<longmapsto> R\<heavy_comma> H'\<heavy_comma> \<medium_left_bracket> OBJ X \<medium_right_bracket> \<^bold>w\<^bold>i\<^bold>t\<^bold>h P \<medium_right_bracket>: G"
+  \<Longrightarrow> \<^bold>s\<^bold>u\<^bold>b\<^bold>t\<^bold>y\<^bold>p\<^bold>e R\<heavy_comma> OBJ H \<longmapsto> R\<heavy_comma> H'\<heavy_comma> \<blangle> OBJ X \<brangle> \<^bold>w\<^bold>i\<^bold>t\<^bold>h P \<^bold>@\<^bold>G\<^bold>O\<^bold>A\<^bold>L G"
   unfolding cast_def
   by (simp add: \<phi>expns times_list_def del: split_paired_All split_paired_Ex)  (metis mult.assoc)
 
 
-lemma [\<phi>reason 70 on \<open>\<medium_left_bracket> \<^bold>s\<^bold>u\<^bold>b\<^bold>t\<^bold>y\<^bold>p\<^bold>e ?R \<heavy_comma> OBJ ?H \<longmapsto> ?R''' \<heavy_comma> \<medium_left_bracket> OBJ ?X \<medium_right_bracket> \<^bold>w\<^bold>i\<^bold>t\<^bold>h ?P \<medium_right_bracket>: ?G\<close>]: \<comment> \<open>or attempts the next cell, if still not succeeded\<close>
+lemma [\<phi>reason 70 on \<open>\<^bold>s\<^bold>u\<^bold>b\<^bold>t\<^bold>y\<^bold>p\<^bold>e ?R \<heavy_comma> OBJ ?H \<longmapsto> ?R''' \<heavy_comma> \<blangle> OBJ ?X \<brangle> \<^bold>w\<^bold>i\<^bold>t\<^bold>h ?P \<^bold>@\<^bold>G\<^bold>O\<^bold>A\<^bold>L ?G\<close>]: \<comment> \<open>or attempts the next cell, if still not succeeded\<close>
   " CHK_SUBGOAL G
-  \<Longrightarrow> \<medium_left_bracket> \<^bold>s\<^bold>u\<^bold>b\<^bold>t\<^bold>y\<^bold>p\<^bold>e R \<longmapsto> R' \<heavy_comma> \<medium_left_bracket> OBJ X \<medium_right_bracket> \<^bold>w\<^bold>i\<^bold>t\<^bold>h P \<medium_right_bracket>: G
-  \<Longrightarrow> \<medium_left_bracket> \<^bold>s\<^bold>u\<^bold>b\<^bold>t\<^bold>y\<^bold>p\<^bold>e R \<heavy_comma> OBJ H \<longmapsto> R' \<heavy_comma> OBJ H \<heavy_comma> \<medium_left_bracket> OBJ X \<medium_right_bracket> \<^bold>w\<^bold>i\<^bold>t\<^bold>h P \<medium_right_bracket>: G "
+  \<Longrightarrow> \<^bold>s\<^bold>u\<^bold>b\<^bold>t\<^bold>y\<^bold>p\<^bold>e R \<longmapsto> R' \<heavy_comma> \<blangle> OBJ X \<brangle> \<^bold>w\<^bold>i\<^bold>t\<^bold>h P \<^bold>@\<^bold>G\<^bold>O\<^bold>A\<^bold>L G
+  \<Longrightarrow> \<^bold>s\<^bold>u\<^bold>b\<^bold>t\<^bold>y\<^bold>p\<^bold>e R \<heavy_comma> OBJ H \<longmapsto> R' \<heavy_comma> OBJ H \<heavy_comma> \<blangle> OBJ X \<brangle> \<^bold>w\<^bold>i\<^bold>t\<^bold>h P \<^bold>@\<^bold>G\<^bold>O\<^bold>A\<^bold>L G "
   unfolding cast_def pair_forall
   by (simp add: \<phi>expns times_list_def) (metis fun_mult_norm mult.commute)
 
@@ -1775,29 +1816,29 @@ lemma [\<phi>reason 10 on \<open>\<^bold>s\<^bold>u\<^bold>b\<^bold>t\<^bold>y\<
    \<^bold>s\<^bold>u\<^bold>b\<^bold>t\<^bold>y\<^bold>p\<^bold>e OBJ a \<Zinj> x \<Ztypecolon> T \<longmapsto> 1 \<heavy_comma> OBJ a' \<Zinj> x' \<Ztypecolon> T' \<^bold>w\<^bold>i\<^bold>t\<^bold>h P"
   unfolding cast_def pair_forall by (simp add: \<phi>expns) blast
 
-lemma [\<phi>reason 1200 on \<open>\<medium_left_bracket> \<^bold>s\<^bold>u\<^bold>b\<^bold>t\<^bold>y\<^bold>p\<^bold>e ?R \<heavy_comma> VAL ?V \<longmapsto> ?R''' \<heavy_comma> \<medium_left_bracket> OBJ ?X \<medium_right_bracket> \<^bold>w\<^bold>i\<^bold>t\<^bold>h ?P \<medium_right_bracket>: ?G\<close>]:
-  " \<medium_left_bracket> \<^bold>s\<^bold>u\<^bold>b\<^bold>t\<^bold>y\<^bold>p\<^bold>e R \<longmapsto> R' \<heavy_comma> \<medium_left_bracket> OBJ X \<medium_right_bracket> \<^bold>w\<^bold>i\<^bold>t\<^bold>h P \<medium_right_bracket>: G
-  \<Longrightarrow> \<medium_left_bracket> \<^bold>s\<^bold>u\<^bold>b\<^bold>t\<^bold>y\<^bold>p\<^bold>e R \<heavy_comma> VAL V \<longmapsto> R' \<heavy_comma> VAL V \<heavy_comma> \<medium_left_bracket> OBJ X \<medium_right_bracket> \<^bold>w\<^bold>i\<^bold>t\<^bold>h P \<medium_right_bracket>: G"
+lemma [\<phi>reason 1200 on \<open>\<^bold>s\<^bold>u\<^bold>b\<^bold>t\<^bold>y\<^bold>p\<^bold>e ?R \<heavy_comma> VAL ?V \<longmapsto> ?R''' \<heavy_comma> \<blangle> OBJ ?X \<brangle> \<^bold>w\<^bold>i\<^bold>t\<^bold>h ?P \<^bold>@\<^bold>G\<^bold>O\<^bold>A\<^bold>L ?G\<close>]:
+  " \<^bold>s\<^bold>u\<^bold>b\<^bold>t\<^bold>y\<^bold>p\<^bold>e R \<longmapsto> R' \<heavy_comma> \<blangle> OBJ X \<brangle> \<^bold>w\<^bold>i\<^bold>t\<^bold>h P \<^bold>@\<^bold>G\<^bold>O\<^bold>A\<^bold>L G
+  \<Longrightarrow> \<^bold>s\<^bold>u\<^bold>b\<^bold>t\<^bold>y\<^bold>p\<^bold>e R \<heavy_comma> VAL V \<longmapsto> R' \<heavy_comma> VAL V \<heavy_comma> \<blangle> OBJ X \<brangle> \<^bold>w\<^bold>i\<^bold>t\<^bold>h P \<^bold>@\<^bold>G\<^bold>O\<^bold>A\<^bold>L G"
   unfolding cast_def pair_forall
   by (simp add: \<phi>expns times_list_def) metis 
 
-lemma [\<phi>reason 2000 on \<open>\<medium_left_bracket> \<^bold>s\<^bold>u\<^bold>b\<^bold>t\<^bold>y\<^bold>p\<^bold>e ?R \<longmapsto> \<medium_left_bracket> ?R2 \<heavy_comma> OBJ ?X \<medium_right_bracket> \<^bold>w\<^bold>i\<^bold>t\<^bold>h ?P \<medium_right_bracket>: ?G\<close>]:
+lemma [\<phi>reason 2000 on \<open>\<^bold>s\<^bold>u\<^bold>b\<^bold>t\<^bold>y\<^bold>p\<^bold>e ?R \<longmapsto> \<blangle> ?R2 \<heavy_comma> OBJ ?X \<brangle> \<^bold>w\<^bold>i\<^bold>t\<^bold>h ?P \<^bold>@\<^bold>G\<^bold>O\<^bold>A\<^bold>L ?G\<close>]:
   " SUBGOAL G G2 \<comment> \<open>make a new subgoal \<close>
-\<Longrightarrow> \<medium_left_bracket> \<^bold>s\<^bold>u\<^bold>b\<^bold>t\<^bold>y\<^bold>p\<^bold>e R \<longmapsto> R1 \<heavy_comma> \<medium_left_bracket> OBJ X \<medium_right_bracket> \<^bold>w\<^bold>i\<^bold>t\<^bold>h P1 \<medium_right_bracket>: G2
+\<Longrightarrow> \<^bold>s\<^bold>u\<^bold>b\<^bold>t\<^bold>y\<^bold>p\<^bold>e R \<longmapsto> R1 \<heavy_comma> \<blangle> OBJ X \<brangle> \<^bold>w\<^bold>i\<^bold>t\<^bold>h P1 \<^bold>@\<^bold>G\<^bold>O\<^bold>A\<^bold>L G2
 \<Longrightarrow> SOLVE_SUBGOAL G2
-\<Longrightarrow> \<medium_left_bracket> \<^bold>s\<^bold>u\<^bold>b\<^bold>t\<^bold>y\<^bold>p\<^bold>e R1 \<longmapsto> \<medium_left_bracket> R2 \<medium_right_bracket> \<^bold>w\<^bold>i\<^bold>t\<^bold>h P2 \<medium_right_bracket>: G
-\<Longrightarrow> \<medium_left_bracket> \<^bold>s\<^bold>u\<^bold>b\<^bold>t\<^bold>y\<^bold>p\<^bold>e R \<longmapsto> \<medium_left_bracket> R2 \<heavy_comma> OBJ X \<medium_right_bracket> \<^bold>w\<^bold>i\<^bold>t\<^bold>h P1 \<and> P2 \<medium_right_bracket>: G"
+\<Longrightarrow> \<^bold>s\<^bold>u\<^bold>b\<^bold>t\<^bold>y\<^bold>p\<^bold>e R1 \<longmapsto> \<blangle> R2 \<brangle> \<^bold>w\<^bold>i\<^bold>t\<^bold>h P2 \<^bold>@\<^bold>G\<^bold>O\<^bold>A\<^bold>L G
+\<Longrightarrow> \<^bold>s\<^bold>u\<^bold>b\<^bold>t\<^bold>y\<^bold>p\<^bold>e R \<longmapsto> \<blangle> R2 \<heavy_comma> OBJ X \<brangle> \<^bold>w\<^bold>i\<^bold>t\<^bold>h P1 \<and> P2 \<^bold>@\<^bold>G\<^bold>O\<^bold>A\<^bold>L G"
   unfolding cast_def pair_forall
   by (simp add: \<phi>expns) blast
 
   
 (* lemma [\<phi>reason 1200
-    on \<open>\<medium_left_bracket> \<^bold>s\<^bold>u\<^bold>b\<^bold>t\<^bold>y\<^bold>p\<^bold>e ?R \<longmapsto> ?R' \<heavy_comma> \<medium_left_bracket> OBJ ?a \<Zinj> ?x \<Ztypecolon> ?X \<medium_right_bracket> \<^bold>w\<^bold>i\<^bold>t\<^bold>h ?P \<^bold>d\<^bold>u\<^bold>a\<^bold>l ?R'\<^sub>m \<heavy_comma> VAL ?V \<heavy_comma> \<medium_left_bracket> OBJ ?a\<^sub>m \<Zinj> ?x\<^sub>m \<Ztypecolon> ?X\<^sub>m \<medium_right_bracket> \<longmapsto> ?R\<^sub>m \<medium_right_bracket>: ?G\<close>
+    on \<open>\<^bold>s\<^bold>u\<^bold>b\<^bold>t\<^bold>y\<^bold>p\<^bold>e ?R \<longmapsto> ?R' \<heavy_comma> \<blangle> OBJ ?a \<Zinj> ?x \<Ztypecolon> ?X \<brangle> \<^bold>w\<^bold>i\<^bold>t\<^bold>h ?P \<^bold>d\<^bold>u\<^bold>a\<^bold>l ?R'\<^sub>m \<heavy_comma> VAL ?V \<heavy_comma> \<blangle> OBJ ?a\<^sub>m \<Zinj> ?x\<^sub>m \<Ztypecolon> ?X\<^sub>m \<brangle> \<longmapsto> ?R\<^sub>m \<^bold>@\<^bold>G\<^bold>O\<^bold>A\<^bold>L ?G\<close>
   ]: \<comment> \<open>OR search the later cells, if hasn't succeeded.\<close>
   "CHK_SUBGOAL G
-    \<Longrightarrow> \<medium_left_bracket> \<^bold>s\<^bold>u\<^bold>b\<^bold>t\<^bold>y\<^bold>p\<^bold>e R \<longmapsto> R' \<heavy_comma> \<medium_left_bracket> OBJ a \<Zinj> x \<Ztypecolon> X \<medium_right_bracket> \<^bold>w\<^bold>i\<^bold>t\<^bold>h P \<^bold>d\<^bold>u\<^bold>a\<^bold>l R'\<^sub>m \<heavy_comma> \<medium_left_bracket> OBJ a\<^sub>m \<Zinj> x\<^sub>m \<Ztypecolon> X\<^sub>m \<medium_right_bracket> \<longmapsto> R\<^sub>m \<medium_right_bracket>: G
-    \<Longrightarrow> \<medium_left_bracket> \<^bold>s\<^bold>u\<^bold>b\<^bold>t\<^bold>y\<^bold>p\<^bold>e R \<longmapsto> R' \<heavy_comma> \<medium_left_bracket> OBJ a \<Zinj> x \<Ztypecolon> X \<medium_right_bracket> \<^bold>w\<^bold>i\<^bold>t\<^bold>h P \<^bold>d\<^bold>u\<^bold>a\<^bold>l R'\<^sub>m \<heavy_comma> VAL V \<heavy_comma> \<medium_left_bracket> OBJ a\<^sub>m \<Zinj> x\<^sub>m \<Ztypecolon> X\<^sub>m \<medium_right_bracket> \<longmapsto> R\<^sub>m \<heavy_comma> VAL V \<medium_right_bracket>: G"
-  unfolding Subty_Target_def Subty_Target2_def Separation_assoc[symmetric]
+    \<Longrightarrow> \<^bold>s\<^bold>u\<^bold>b\<^bold>t\<^bold>y\<^bold>p\<^bold>e R \<longmapsto> R' \<heavy_comma> \<blangle> OBJ a \<Zinj> x \<Ztypecolon> X \<brangle> \<^bold>w\<^bold>i\<^bold>t\<^bold>h P \<^bold>d\<^bold>u\<^bold>a\<^bold>l R'\<^sub>m \<heavy_comma> \<blangle> OBJ a\<^sub>m \<Zinj> x\<^sub>m \<Ztypecolon> X\<^sub>m \<brangle> \<longmapsto> R\<^sub>m \<^bold>@\<^bold>G\<^bold>O\<^bold>A\<^bold>L G
+    \<Longrightarrow> \<^bold>s\<^bold>u\<^bold>b\<^bold>t\<^bold>y\<^bold>p\<^bold>e R \<longmapsto> R' \<heavy_comma> \<blangle> OBJ a \<Zinj> x \<Ztypecolon> X \<brangle> \<^bold>w\<^bold>i\<^bold>t\<^bold>h P \<^bold>d\<^bold>u\<^bold>a\<^bold>l R'\<^sub>m \<heavy_comma> VAL V \<heavy_comma> \<blangle> OBJ a\<^sub>m \<Zinj> x\<^sub>m \<Ztypecolon> X\<^sub>m \<brangle> \<longmapsto> R\<^sub>m \<heavy_comma> VAL V \<^bold>@\<^bold>G\<^bold>O\<^bold>A\<^bold>L G"
+  unfolding FOCUS_TAG_def Subty_Target2_def Separation_assoc[symmetric]
     Separation_comm(2)[of "VAL V" "\<tort_lbrace>a\<^sub>m \<Zinj> x\<^sub>m \<Ztypecolon> X\<^sub>m\<tort_rbrace>"]
   unfolding Separation_assoc
   by (rule cast_dual_intro_frame_R[where M = 1, unfolded Separation_empty])
@@ -1807,17 +1848,17 @@ text \<open>step cases when the reasoner faces an object argument \<^term>\<open
 
 subsubsection \<open>Ordered\<close>
 
-lemma [\<phi>reason 2000 on \<open>\<medium_left_bracket> \<^bold>s\<^bold>u\<^bold>b\<^bold>t\<^bold>y\<^bold>p\<^bold>e ?R\<heavy_comma> VAL ?Y \<longmapsto> \<medium_left_bracket> ?R2 \<heavy_comma> (FIX VAL ?X) \<medium_right_bracket> \<^bold>w\<^bold>i\<^bold>t\<^bold>h ?P \<medium_right_bracket>: ?G\<close>]:
+lemma [\<phi>reason 2000 on \<open>\<^bold>s\<^bold>u\<^bold>b\<^bold>t\<^bold>y\<^bold>p\<^bold>e ?R\<heavy_comma> VAL ?Y \<longmapsto> \<blangle> ?R2 \<heavy_comma> (FIX VAL ?X) \<brangle> \<^bold>w\<^bold>i\<^bold>t\<^bold>h ?P \<^bold>@\<^bold>G\<^bold>O\<^bold>A\<^bold>L ?G\<close>]:
   " \<^bold>s\<^bold>u\<^bold>b\<^bold>t\<^bold>y\<^bold>p\<^bold>e Y \<longmapsto> X \<^bold>w\<^bold>i\<^bold>t\<^bold>h P1
-\<Longrightarrow> \<medium_left_bracket> \<^bold>s\<^bold>u\<^bold>b\<^bold>t\<^bold>y\<^bold>p\<^bold>e R \<longmapsto> \<medium_left_bracket> R2 \<medium_right_bracket> \<^bold>w\<^bold>i\<^bold>t\<^bold>h P2 \<medium_right_bracket>: G
-\<Longrightarrow> \<medium_left_bracket> \<^bold>s\<^bold>u\<^bold>b\<^bold>t\<^bold>y\<^bold>p\<^bold>e R\<heavy_comma> VAL Y \<longmapsto> \<medium_left_bracket> R2 \<heavy_comma> FIX VAL X \<medium_right_bracket> \<^bold>w\<^bold>i\<^bold>t\<^bold>h P1 \<and> P2 \<medium_right_bracket>: G"
+\<Longrightarrow> \<^bold>s\<^bold>u\<^bold>b\<^bold>t\<^bold>y\<^bold>p\<^bold>e R \<longmapsto> \<blangle> R2 \<brangle> \<^bold>w\<^bold>i\<^bold>t\<^bold>h P2 \<^bold>@\<^bold>G\<^bold>O\<^bold>A\<^bold>L G
+\<Longrightarrow> \<^bold>s\<^bold>u\<^bold>b\<^bold>t\<^bold>y\<^bold>p\<^bold>e R\<heavy_comma> VAL Y \<longmapsto> \<blangle> R2 \<heavy_comma> FIX VAL X \<brangle> \<^bold>w\<^bold>i\<^bold>t\<^bold>h P1 \<and> P2 \<^bold>@\<^bold>G\<^bold>O\<^bold>A\<^bold>L G"
   unfolding cast_def pair_forall
   by (simp add: \<phi>expns) metis
 
-lemma [\<phi>reason 2000 on \<open>\<medium_left_bracket> \<^bold>s\<^bold>u\<^bold>b\<^bold>t\<^bold>y\<^bold>p\<^bold>e ?R \<heavy_comma> OBJ ?Y \<longmapsto> \<medium_left_bracket> ?R2\<heavy_comma> FIX OBJ ?X \<medium_right_bracket> \<^bold>w\<^bold>i\<^bold>t\<^bold>h ?P \<medium_right_bracket>: ?G\<close>]:
+lemma [\<phi>reason 2000 on \<open>\<^bold>s\<^bold>u\<^bold>b\<^bold>t\<^bold>y\<^bold>p\<^bold>e ?R \<heavy_comma> OBJ ?Y \<longmapsto> \<blangle> ?R2\<heavy_comma> FIX OBJ ?X \<brangle> \<^bold>w\<^bold>i\<^bold>t\<^bold>h ?P \<^bold>@\<^bold>G\<^bold>O\<^bold>A\<^bold>L ?G\<close>]:
   " \<^bold>s\<^bold>u\<^bold>b\<^bold>t\<^bold>y\<^bold>p\<^bold>e Y \<longmapsto> X \<^bold>w\<^bold>i\<^bold>t\<^bold>h P
-\<Longrightarrow> \<medium_left_bracket> \<^bold>s\<^bold>u\<^bold>b\<^bold>t\<^bold>y\<^bold>p\<^bold>e R \<longmapsto> \<medium_left_bracket> R2 \<medium_right_bracket> \<^bold>w\<^bold>i\<^bold>t\<^bold>h P2 \<medium_right_bracket>: G
-\<Longrightarrow> \<medium_left_bracket> \<^bold>s\<^bold>u\<^bold>b\<^bold>t\<^bold>y\<^bold>p\<^bold>e R\<heavy_comma> OBJ Y \<longmapsto> \<medium_left_bracket> R2\<heavy_comma> FIX OBJ X \<medium_right_bracket> \<^bold>w\<^bold>i\<^bold>t\<^bold>h P \<and> P2 \<medium_right_bracket>: G"
+\<Longrightarrow> \<^bold>s\<^bold>u\<^bold>b\<^bold>t\<^bold>y\<^bold>p\<^bold>e R \<longmapsto> \<blangle> R2 \<brangle> \<^bold>w\<^bold>i\<^bold>t\<^bold>h P2 \<^bold>@\<^bold>G\<^bold>O\<^bold>A\<^bold>L G
+\<Longrightarrow> \<^bold>s\<^bold>u\<^bold>b\<^bold>t\<^bold>y\<^bold>p\<^bold>e R\<heavy_comma> OBJ Y \<longmapsto> \<blangle> R2\<heavy_comma> FIX OBJ X \<brangle> \<^bold>w\<^bold>i\<^bold>t\<^bold>h P \<and> P2 \<^bold>@\<^bold>G\<^bold>O\<^bold>A\<^bold>L G"
   unfolding cast_def Fix_def
   by (simp add: \<phi>expns times_list_def) blast
 
@@ -1825,13 +1866,13 @@ lemma [\<phi>reason 2000 on \<open>\<medium_left_bracket> \<^bold>s\<^bold>u\<^b
 subsubsection \<open>Plainize\<close>
 
 lemma [\<phi>reason 2000]:
-  "\<medium_left_bracket> \<^bold>s\<^bold>u\<^bold>b\<^bold>t\<^bold>y\<^bold>p\<^bold>e R \<heavy_comma> T1 \<heavy_comma> T2 \<longmapsto> X \<^bold>w\<^bold>i\<^bold>t\<^bold>h P \<medium_right_bracket>: G
-  \<Longrightarrow> \<medium_left_bracket> \<^bold>s\<^bold>u\<^bold>b\<^bold>t\<^bold>y\<^bold>p\<^bold>e R \<heavy_comma> (T1 \<heavy_comma> T2) \<longmapsto> X \<^bold>w\<^bold>i\<^bold>t\<^bold>h P \<medium_right_bracket>: G"
+  "\<^bold>s\<^bold>u\<^bold>b\<^bold>t\<^bold>y\<^bold>p\<^bold>e R \<heavy_comma> T1 \<heavy_comma> T2 \<longmapsto> X \<^bold>w\<^bold>i\<^bold>t\<^bold>h P \<^bold>@\<^bold>G\<^bold>O\<^bold>A\<^bold>L G
+  \<Longrightarrow> \<^bold>s\<^bold>u\<^bold>b\<^bold>t\<^bold>y\<^bold>p\<^bold>e R \<heavy_comma> (T1 \<heavy_comma> T2) \<longmapsto> X \<^bold>w\<^bold>i\<^bold>t\<^bold>h P \<^bold>@\<^bold>G\<^bold>O\<^bold>A\<^bold>L G"
   unfolding mult.assoc[symmetric] .
 
 lemma [\<phi>reason 2000]:
-  "\<medium_left_bracket> \<^bold>s\<^bold>u\<^bold>b\<^bold>t\<^bold>y\<^bold>p\<^bold>e T \<longmapsto> \<medium_left_bracket> R \<heavy_comma> X1 \<heavy_comma> X2 \<medium_right_bracket> \<^bold>w\<^bold>i\<^bold>t\<^bold>h P \<medium_right_bracket>: G
-  \<Longrightarrow> \<medium_left_bracket> \<^bold>s\<^bold>u\<^bold>b\<^bold>t\<^bold>y\<^bold>p\<^bold>e T \<longmapsto> \<medium_left_bracket> R \<heavy_comma> (X1 \<heavy_comma> X2) \<medium_right_bracket> \<^bold>w\<^bold>i\<^bold>t\<^bold>h P \<medium_right_bracket>: G"
+  "\<^bold>s\<^bold>u\<^bold>b\<^bold>t\<^bold>y\<^bold>p\<^bold>e T \<longmapsto> \<blangle> R \<heavy_comma> X1 \<heavy_comma> X2 \<brangle> \<^bold>w\<^bold>i\<^bold>t\<^bold>h P \<^bold>@\<^bold>G\<^bold>O\<^bold>A\<^bold>L G
+  \<Longrightarrow> \<^bold>s\<^bold>u\<^bold>b\<^bold>t\<^bold>y\<^bold>p\<^bold>e T \<longmapsto> \<blangle> R \<heavy_comma> (X1 \<heavy_comma> X2) \<brangle> \<^bold>w\<^bold>i\<^bold>t\<^bold>h P \<^bold>@\<^bold>G\<^bold>O\<^bold>A\<^bold>L G"
   unfolding mult.assoc[symmetric] .
 
 end
@@ -1840,20 +1881,20 @@ end
 subsection \<open>Scan\<close>
 
 lemma [\<phi>intro 110]:
-  "\<medium_left_bracket> \<^bold>s\<^bold>u\<^bold>b\<^bold>t\<^bold>y\<^bold>p\<^bold>e R \<longmapsto> R' * \<medium_left_bracket> VAL X \<medium_right_bracket> \<^bold>w\<^bold>i\<^bold>t\<^bold>h P \<medium_right_bracket>
-  \<Longrightarrow> \<medium_left_bracket> \<^bold>s\<^bold>u\<^bold>b\<^bold>t\<^bold>y\<^bold>p\<^bold>e L * R \<longmapsto> L * R' * \<medium_left_bracket> VAL X \<medium_right_bracket> \<^bold>w\<^bold>i\<^bold>t\<^bold>h P \<medium_right_bracket>"
+  "\<^bold>s\<^bold>u\<^bold>b\<^bold>t\<^bold>y\<^bold>p\<^bold>e R \<longmapsto> R' * \<blangle> VAL X \<brangle> \<^bold>w\<^bold>i\<^bold>t\<^bold>h P \<brangle>
+  \<Longrightarrow> \<^bold>s\<^bold>u\<^bold>b\<^bold>t\<^bold>y\<^bold>p\<^bold>e L * R \<longmapsto> L * R' * \<blangle> VAL X \<brangle> \<^bold>w\<^bold>i\<^bold>t\<^bold>h P \<brangle>"
   unfolding cast_def Intro_def Dest_def pair_forall
   by (metis Separation_assoc Separation_expn)
 
 lemma [\<phi>intro 110]:
-  "\<medium_left_bracket> \<^bold>s\<^bold>u\<^bold>b\<^bold>t\<^bold>y\<^bold>p\<^bold>e R \<longmapsto> R' * \<medium_left_bracket> OBJ X \<medium_right_bracket> \<^bold>w\<^bold>i\<^bold>t\<^bold>h P \<medium_right_bracket>
-  \<Longrightarrow> \<medium_left_bracket> \<^bold>s\<^bold>u\<^bold>b\<^bold>t\<^bold>y\<^bold>p\<^bold>e L * R \<longmapsto> L * R' * \<medium_left_bracket> OBJ X \<medium_right_bracket> \<^bold>w\<^bold>i\<^bold>t\<^bold>h P \<medium_right_bracket>"
+  "\<^bold>s\<^bold>u\<^bold>b\<^bold>t\<^bold>y\<^bold>p\<^bold>e R \<longmapsto> R' * \<blangle> OBJ X \<brangle> \<^bold>w\<^bold>i\<^bold>t\<^bold>h P \<brangle>
+  \<Longrightarrow> \<^bold>s\<^bold>u\<^bold>b\<^bold>t\<^bold>y\<^bold>p\<^bold>e L * R \<longmapsto> L * R' * \<blangle> OBJ X \<brangle> \<^bold>w\<^bold>i\<^bold>t\<^bold>h P \<brangle>"
   unfolding cast_def Intro_def Dest_def pair_forall
   by (metis Separation_assoc Separation_expn)
 
 lemma [\<phi>intro 100]:
-  "\<medium_left_bracket> \<^bold>s\<^bold>u\<^bold>b\<^bold>t\<^bold>y\<^bold>p\<^bold>e L \<longmapsto> L' * \<medium_left_bracket> x \<Ztypecolon> X \<medium_right_bracket> \<^bold>w\<^bold>i\<^bold>t\<^bold>h P \<medium_right_bracket>
-  \<Longrightarrow> \<medium_left_bracket> \<^bold>s\<^bold>u\<^bold>b\<^bold>t\<^bold>y\<^bold>p\<^bold>e H * R \<longmapsto> H' * R * \<medium_left_bracket> x \<Ztypecolon> X \<medium_right_bracket> \<^bold>w\<^bold>i\<^bold>t\<^bold>h P \<medium_right_bracket>"
+  "\<^bold>s\<^bold>u\<^bold>b\<^bold>t\<^bold>y\<^bold>p\<^bold>e L \<longmapsto> L' * \<blangle> x \<Ztypecolon> X \<brangle> \<^bold>w\<^bold>i\<^bold>t\<^bold>h P \<brangle>
+  \<Longrightarrow> \<^bold>s\<^bold>u\<^bold>b\<^bold>t\<^bold>y\<^bold>p\<^bold>e H * R \<longmapsto> H' * R * \<blangle> x \<Ztypecolon> X \<brangle> \<^bold>w\<^bold>i\<^bold>t\<^bold>h P \<brangle>"
   unfolding Subty_def SubtyDual_def Heap_Subty_Goal_def Intro_def Dest_def
     Separation_comm[of H R] Separation_comm[of H' R]
   by (metis Heap_Divider_exps Separation_assoc)
@@ -1866,8 +1907,8 @@ lemma [\<phi>intro 100]:
 
 
 lemma heap_idx_R_dual[\<phi>intro 100]:
-  "\<medium_left_bracket> \<^bold>s\<^bold>u\<^bold>b\<^bold>t\<^bold>y\<^bold>p\<^bold>e H \<longmapsto> H' * \<medium_left_bracket> x \<Ztypecolon> X \<medium_right_bracket> \<^bold>w\<^bold>i\<^bold>t\<^bold>h P \<^bold>d\<^bold>u\<^bold>a\<^bold>l H'\<^sub>m * \<medium_left_bracket> x\<^sub>m \<Ztypecolon> X\<^sub>m \<medium_right_bracket> \<longmapsto> H\<^sub>m \<medium_right_bracket>
-  \<Longrightarrow> \<medium_left_bracket> \<^bold>s\<^bold>u\<^bold>b\<^bold>t\<^bold>y\<^bold>p\<^bold>e H * R \<longmapsto> H' * R * \<medium_left_bracket> x \<Ztypecolon> X \<medium_right_bracket> \<^bold>w\<^bold>i\<^bold>t\<^bold>h P \<^bold>d\<^bold>u\<^bold>a\<^bold>l H'\<^sub>m * R * \<medium_left_bracket> x\<^sub>m \<Ztypecolon> X\<^sub>m \<medium_right_bracket> \<longmapsto> H\<^sub>m * R \<medium_right_bracket>"
+  "\<^bold>s\<^bold>u\<^bold>b\<^bold>t\<^bold>y\<^bold>p\<^bold>e H \<longmapsto> H' * \<blangle> x \<Ztypecolon> X \<brangle> \<^bold>w\<^bold>i\<^bold>t\<^bold>h P \<^bold>d\<^bold>u\<^bold>a\<^bold>l H'\<^sub>m * \<blangle> x\<^sub>m \<Ztypecolon> X\<^sub>m \<brangle> \<longmapsto> H\<^sub>m \<brangle>
+  \<Longrightarrow> \<^bold>s\<^bold>u\<^bold>b\<^bold>t\<^bold>y\<^bold>p\<^bold>e H * R \<longmapsto> H' * R * \<blangle> x \<Ztypecolon> X \<brangle> \<^bold>w\<^bold>i\<^bold>t\<^bold>h P \<^bold>d\<^bold>u\<^bold>a\<^bold>l H'\<^sub>m * R * \<blangle> x\<^sub>m \<Ztypecolon> X\<^sub>m \<brangle> \<longmapsto> H\<^sub>m * R \<brangle>"
   unfolding Subty_def SubtyDual_def Heap_Subty_Goal_def Intro_def Dest_def
     Separation_comm[of H R] Separation_comm[of H\<^sub>m R]
     Separation_comm[of H' R] Separation_comm[of H'\<^sub>m R]
@@ -1877,23 +1918,23 @@ lemma heap_idx_R_dual[\<phi>intro 100]:
 
 
 lemma [\<phi>intro 120]:
-  "\<medium_left_bracket> \<^bold>s\<^bold>u\<^bold>b\<^bold>t\<^bold>y\<^bold>p\<^bold>e H \<longmapsto> H1 * x \<Ztypecolon> \<medium_left_bracket> X \<medium_right_bracket> \<^bold>w\<^bold>i\<^bold>t\<^bold>h P1 \<medium_right_bracket>
-    \<Longrightarrow> (P1 \<Longrightarrow> \<medium_left_bracket> \<^bold>s\<^bold>u\<^bold>b\<^bold>t\<^bold>y\<^bold>p\<^bold>e H1 \<longmapsto> H\<^sub>r * h2 \<Ztypecolon> \<medium_left_bracket> H2 \<medium_right_bracket> \<^bold>w\<^bold>i\<^bold>t\<^bold>h P2 \<medium_right_bracket>)
-    \<Longrightarrow> \<medium_left_bracket> \<^bold>s\<^bold>u\<^bold>b\<^bold>t\<^bold>y\<^bold>p\<^bold>e H \<longmapsto> H\<^sub>r * (x, h2) \<Ztypecolon> \<medium_left_bracket> X \<^emph> H2 \<medium_right_bracket> \<^bold>w\<^bold>i\<^bold>t\<^bold>h P1 \<and> P2 \<medium_right_bracket>"
+  "\<^bold>s\<^bold>u\<^bold>b\<^bold>t\<^bold>y\<^bold>p\<^bold>e H \<longmapsto> H1 * x \<Ztypecolon> \<blangle> X \<brangle> \<^bold>w\<^bold>i\<^bold>t\<^bold>h P1 \<brangle>
+    \<Longrightarrow> (P1 \<Longrightarrow> \<^bold>s\<^bold>u\<^bold>b\<^bold>t\<^bold>y\<^bold>p\<^bold>e H1 \<longmapsto> H\<^sub>r * h2 \<Ztypecolon> \<blangle> H2 \<brangle> \<^bold>w\<^bold>i\<^bold>t\<^bold>h P2 \<brangle>)
+    \<Longrightarrow> \<^bold>s\<^bold>u\<^bold>b\<^bold>t\<^bold>y\<^bold>p\<^bold>e H \<longmapsto> H\<^sub>r * (x, h2) \<Ztypecolon> \<blangle> X \<^emph> H2 \<brangle> \<^bold>w\<^bold>i\<^bold>t\<^bold>h P1 \<and> P2 \<brangle>"
   unfolding Subty_def SubtyDual_def Heap_Subty_Goal_def HeapDivNu_to_SepSet SepNu_to_SepSet Intro_def Dest_def
   by (smt (verit, del_insts) SeparationSet_assoc SeparationSet_comm SeparationSet_def mem_Collect_eq)
 *)
 (* lemma [ \<phi>intro -50 ]: "\<^bold>d\<^bold>e\<^bold>s\<^bold>t \<^bold>s\<^bold>u\<^bold>b\<^bold>t\<^bold>y\<^bold>p\<^bold>e x \<Ztypecolon> T \<longmapsto> d \<Ztypecolon> D \<^bold>w\<^bold>i\<^bold>t\<^bold>h P
-  \<Longrightarrow> (P \<Longrightarrow> \<medium_left_bracket> \<^bold>s\<^bold>u\<^bold>b\<^bold>t\<^bold>y\<^bold>p\<^bold>e d \<Ztypecolon> D \<longmapsto> d' \<Ztypecolon> D' * h \<Ztypecolon> \<medium_left_bracket> H \<medium_right_bracket> \<^bold>w\<^bold>i\<^bold>t\<^bold>h P2 \<^bold>d\<^bold>u\<^bold>a\<^bold>l i'\<^sub>m \<Ztypecolon> I'\<^sub>m * h\<^sub>m \<Ztypecolon> \<medium_left_bracket> H\<^sub>m \<medium_right_bracket> \<longmapsto> i \<Ztypecolon> I \<medium_right_bracket>)
+  \<Longrightarrow> (P \<Longrightarrow> \<^bold>s\<^bold>u\<^bold>b\<^bold>t\<^bold>y\<^bold>p\<^bold>e d \<Ztypecolon> D \<longmapsto> d' \<Ztypecolon> D' * h \<Ztypecolon> \<blangle> H \<brangle> \<^bold>w\<^bold>i\<^bold>t\<^bold>h P2 \<^bold>d\<^bold>u\<^bold>a\<^bold>l i'\<^sub>m \<Ztypecolon> I'\<^sub>m * h\<^sub>m \<Ztypecolon> \<blangle> H\<^sub>m \<brangle> \<longmapsto> i \<Ztypecolon> I \<brangle>)
   \<Longrightarrow> (P \<Longrightarrow> P2 \<Longrightarrow> \<^bold>i\<^bold>n\<^bold>t\<^bold>r\<^bold>o \<^bold>s\<^bold>u\<^bold>b\<^bold>t\<^bold>y\<^bold>p\<^bold>e i \<Ztypecolon> I \<longmapsto> x\<^sub>m \<Ztypecolon> T \<^bold>w\<^bold>i\<^bold>t\<^bold>h Anyway)
-  \<Longrightarrow> \<medium_left_bracket> \<^bold>s\<^bold>u\<^bold>b\<^bold>t\<^bold>y\<^bold>p\<^bold>e x \<Ztypecolon> T \<longmapsto> d' \<Ztypecolon> D' * h \<Ztypecolon> \<medium_left_bracket> H \<medium_right_bracket> \<^bold>w\<^bold>i\<^bold>t\<^bold>h P \<and> P2 \<^bold>d\<^bold>u\<^bold>a\<^bold>l i'\<^sub>m \<Ztypecolon> I'\<^sub>m * h\<^sub>m \<Ztypecolon> \<medium_left_bracket> H\<^sub>m \<medium_right_bracket> \<longmapsto> x\<^sub>m \<Ztypecolon> T \<medium_right_bracket>"
+  \<Longrightarrow> \<^bold>s\<^bold>u\<^bold>b\<^bold>t\<^bold>y\<^bold>p\<^bold>e x \<Ztypecolon> T \<longmapsto> d' \<Ztypecolon> D' * h \<Ztypecolon> \<blangle> H \<brangle> \<^bold>w\<^bold>i\<^bold>t\<^bold>h P \<and> P2 \<^bold>d\<^bold>u\<^bold>a\<^bold>l i'\<^sub>m \<Ztypecolon> I'\<^sub>m * h\<^sub>m \<Ztypecolon> \<blangle> H\<^sub>m \<brangle> \<longmapsto> x\<^sub>m \<Ztypecolon> T \<brangle>"
   unfolding Dest_def Intro_def SubtyDual_def Different_def Heap_Subty_Goal_def Subty_def
   by (auto simp add: Premise_def) *)
 
 (* lemma [ \<phi>intro 50 ]: "\<^bold>s\<^bold>u\<^bold>b\<^bold>t\<^bold>y\<^bold>p\<^bold>e x \<Ztypecolon> T \<longmapsto> d \<Ztypecolon> D \<^bold>w\<^bold>i\<^bold>t\<^bold>h P
-  \<Longrightarrow> (P \<Longrightarrow> \<medium_left_bracket> \<^bold>s\<^bold>u\<^bold>b\<^bold>t\<^bold>y\<^bold>p\<^bold>e d \<Ztypecolon> D \<longmapsto> d' \<Ztypecolon> D' * h \<Ztypecolon> \<medium_left_bracket> H \<medium_right_bracket> \<^bold>w\<^bold>i\<^bold>t\<^bold>h P2 \<^bold>d\<^bold>u\<^bold>a\<^bold>l i'\<^sub>m \<Ztypecolon> I'\<^sub>m * h\<^sub>m \<Ztypecolon> \<medium_left_bracket> H\<^sub>m \<medium_right_bracket> \<longmapsto> i \<Ztypecolon> I \<medium_right_bracket>)
+  \<Longrightarrow> (P \<Longrightarrow> \<^bold>s\<^bold>u\<^bold>b\<^bold>t\<^bold>y\<^bold>p\<^bold>e d \<Ztypecolon> D \<longmapsto> d' \<Ztypecolon> D' * h \<Ztypecolon> \<blangle> H \<brangle> \<^bold>w\<^bold>i\<^bold>t\<^bold>h P2 \<^bold>d\<^bold>u\<^bold>a\<^bold>l i'\<^sub>m \<Ztypecolon> I'\<^sub>m * h\<^sub>m \<Ztypecolon> \<blangle> H\<^sub>m \<brangle> \<longmapsto> i \<Ztypecolon> I \<brangle>)
   \<Longrightarrow> (P \<Longrightarrow> P2 \<Longrightarrow> \<^bold>i\<^bold>n\<^bold>t\<^bold>r\<^bold>o \<^bold>s\<^bold>u\<^bold>b\<^bold>t\<^bold>y\<^bold>p\<^bold>e i \<Ztypecolon> I \<longmapsto> x\<^sub>m \<Ztypecolon> T \<^bold>w\<^bold>i\<^bold>t\<^bold>h Anyway)
-  \<Longrightarrow> \<medium_left_bracket> \<^bold>s\<^bold>u\<^bold>b\<^bold>t\<^bold>y\<^bold>p\<^bold>e x \<Ztypecolon> T \<longmapsto> d' \<Ztypecolon> D' * h \<Ztypecolon> \<medium_left_bracket> H \<medium_right_bracket> \<^bold>w\<^bold>i\<^bold>t\<^bold>h P \<and> P2 \<medium_right_bracket>"
+  \<Longrightarrow> \<^bold>s\<^bold>u\<^bold>b\<^bold>t\<^bold>y\<^bold>p\<^bold>e x \<Ztypecolon> T \<longmapsto> d' \<Ztypecolon> D' * h \<Ztypecolon> \<blangle> H \<brangle> \<^bold>w\<^bold>i\<^bold>t\<^bold>h P \<and> P2 \<brangle>"
   unfolding Dest_def Intro_def SubtyDual_def Different_def Heap_Subty_Goal_def Subty_def
   by (auto simp add: Premise_def) *)
 
@@ -2040,7 +2081,7 @@ subsubsection \<open>Separations Initialization\<close>
 
 lemma [\<phi>reason 1200]:
   "SUBGOAL TOP_GOAL G
-   \<Longrightarrow> \<medium_left_bracket> \<^bold>c\<^bold>o\<^bold>n\<^bold>v Merge P (L1 * L2) (1 * \<medium_left_bracket> R \<medium_right_bracket>) = X \<medium_right_bracket>: G
+   \<Longrightarrow> \<^bold>c\<^bold>o\<^bold>n\<^bold>v Merge P (L1 * L2) (1 * \<blangle> R \<brangle>) = X \<^bold>@\<^bold>G\<^bold>O\<^bold>A\<^bold>L G
    \<Longrightarrow> \<^bold>c\<^bold>o\<^bold>n\<^bold>v Merge P (L1 * L2) R = X"
   for X :: \<open>'a::monoid_mult set\<close>
   unfolding Conv_def cast_def mult_1_left . 
@@ -2052,16 +2093,16 @@ lemma [\<phi>reason 1200 on \<open>\<^bold>c\<^bold>o\<^bold>n\<^bold>v Merge ?P
    \<Longrightarrow> \<^bold>c\<^bold>o\<^bold>n\<^bold>v Merge P (VAL V1) (VAL V2) = (VAL V)"
   unfolding Conv_def cast_def Merge_def by force
 
-lemma (in std) [\<phi>reason 1200 on \<open>\<medium_left_bracket> \<^bold>c\<^bold>o\<^bold>n\<^bold>v Merge ?P (?R1 \<heavy_comma> VAL ?V1) (?N \<heavy_comma> \<medium_left_bracket> ?R2 \<heavy_comma> VAL ?V2 \<medium_right_bracket>) = ?X \<medium_right_bracket>: ?G\<close> ]:
+lemma (in std) [\<phi>reason 1200 on \<open>\<^bold>c\<^bold>o\<^bold>n\<^bold>v Merge ?P (?R1 \<heavy_comma> VAL ?V1) (?N \<heavy_comma> \<blangle> ?R2 \<heavy_comma> VAL ?V2 \<brangle>) = ?X \<^bold>@\<^bold>G\<^bold>O\<^bold>A\<^bold>L ?G\<close> ]:
   "\<^bold>c\<^bold>o\<^bold>n\<^bold>v Merge P V1 V2 = V
-   \<Longrightarrow> \<medium_left_bracket> \<^bold>c\<^bold>o\<^bold>n\<^bold>v Merge P R1 (1 \<heavy_comma> \<medium_left_bracket> N \<heavy_comma> R2 \<medium_right_bracket>) = R \<medium_right_bracket>: G
-   \<Longrightarrow> \<medium_left_bracket> \<^bold>c\<^bold>o\<^bold>n\<^bold>v Merge P (R1 \<heavy_comma> VAL V1) (N \<heavy_comma> \<medium_left_bracket> R2 \<heavy_comma> VAL V2 \<medium_right_bracket>) = (R \<heavy_comma> VAL V) \<medium_right_bracket>: G"
+   \<Longrightarrow> \<^bold>c\<^bold>o\<^bold>n\<^bold>v Merge P R1 (1 \<heavy_comma> \<blangle> N \<heavy_comma> R2 \<brangle>) = R \<^bold>@\<^bold>G\<^bold>O\<^bold>A\<^bold>L G
+   \<Longrightarrow> \<^bold>c\<^bold>o\<^bold>n\<^bold>v Merge P (R1 \<heavy_comma> VAL V1) (N \<heavy_comma> \<blangle> R2 \<heavy_comma> VAL V2 \<brangle>) = (R \<heavy_comma> VAL V) \<^bold>@\<^bold>G\<^bold>O\<^bold>A\<^bold>L G"
   unfolding Conv_def cast_def Merge_def
   using mult.assoc by fastforce
 
 lemma (in std) [\<phi>reason 1200]:
-  "\<medium_left_bracket> \<^bold>c\<^bold>o\<^bold>n\<^bold>v Merge P (R1 \<heavy_comma> VAL V1) (N \<heavy_comma> OBJ H2 \<heavy_comma> \<medium_left_bracket> R2 \<medium_right_bracket>) = R \<medium_right_bracket>: G
-   \<Longrightarrow> \<medium_left_bracket> \<^bold>c\<^bold>o\<^bold>n\<^bold>v Merge P (R1 \<heavy_comma> VAL V1) (N \<heavy_comma> \<medium_left_bracket> R2 \<heavy_comma> OBJ H2 \<medium_right_bracket>) = R \<medium_right_bracket>: G"
+  "\<^bold>c\<^bold>o\<^bold>n\<^bold>v Merge P (R1 \<heavy_comma> VAL V1) (N \<heavy_comma> OBJ H2 \<heavy_comma> \<blangle> R2 \<brangle>) = R \<^bold>@\<^bold>G\<^bold>O\<^bold>A\<^bold>L G
+   \<Longrightarrow> \<^bold>c\<^bold>o\<^bold>n\<^bold>v Merge P (R1 \<heavy_comma> VAL V1) (N \<heavy_comma> \<blangle> R2 \<heavy_comma> OBJ H2 \<brangle>) = R \<^bold>@\<^bold>G\<^bold>O\<^bold>A\<^bold>L G"
   unfolding Conv_def cast_def Merge_def
     by (metis mult.assoc OBJ_comm)
 
@@ -2079,93 +2120,93 @@ lemma [\<phi>reason]:
 lemma [\<phi>reason on \<open>\<^bold>c\<^bold>o\<^bold>n\<^bold>v Merge ?P (OBJ ?H1) (OBJ ?H2) = ?X\<close> ]:
   "\<^bold>c\<^bold>o\<^bold>n\<^bold>v Merge P H1 H2 = H
   \<Longrightarrow> \<^bold>c\<^bold>o\<^bold>n\<^bold>v Merge P (OBJ H1) (OBJ H2) = (OBJ H)"
-  unfolding Conv_def Subty_Target_def Merge_def by force
+  unfolding Conv_def FOCUS_TAG_def Merge_def by force
 
 lemma (in std) [\<phi>reason 1200]:
-  "\<medium_left_bracket> \<^bold>c\<^bold>o\<^bold>n\<^bold>v Merge (MergeNeg P) (N \<heavy_comma> R \<heavy_comma> VAL V2) (1 \<heavy_comma> \<medium_left_bracket> L \<heavy_comma> OBJ H1\<medium_right_bracket>) = X \<medium_right_bracket>: G
-   \<Longrightarrow> \<medium_left_bracket> \<^bold>c\<^bold>o\<^bold>n\<^bold>v Merge P (L \<heavy_comma> OBJ H1) (N \<heavy_comma> \<medium_left_bracket> R \<heavy_comma> VAL V2 \<medium_right_bracket>) = X \<medium_right_bracket>: G"
+  "\<^bold>c\<^bold>o\<^bold>n\<^bold>v Merge (MergeNeg P) (N \<heavy_comma> R \<heavy_comma> VAL V2) (1 \<heavy_comma> \<blangle> L \<heavy_comma> OBJ H1\<brangle>) = X \<^bold>@\<^bold>G\<^bold>O\<^bold>A\<^bold>L G
+   \<Longrightarrow> \<^bold>c\<^bold>o\<^bold>n\<^bold>v Merge P (L \<heavy_comma> OBJ H1) (N \<heavy_comma> \<blangle> R \<heavy_comma> VAL V2 \<brangle>) = X \<^bold>@\<^bold>G\<^bold>O\<^bold>A\<^bold>L G"
   unfolding Conv_def cast_def Merge_def MergeNeg_def mult_1_left
   by (metis mult.assoc)
 
 lemma (in std) [\<phi>reason 1200]:
-  "\<medium_left_bracket> \<^bold>c\<^bold>o\<^bold>n\<^bold>v Merge P (N \<heavy_comma> R) (1 \<heavy_comma> \<medium_left_bracket> L \<heavy_comma> OBJ H1\<medium_right_bracket>) = X \<medium_right_bracket>: G
-   \<Longrightarrow> \<medium_left_bracket> \<^bold>c\<^bold>o\<^bold>n\<^bold>v Merge (MergeNeg P) (L \<heavy_comma> OBJ H1) (N \<heavy_comma> \<medium_left_bracket> R \<medium_right_bracket>) = X \<medium_right_bracket>: G"
+  "\<^bold>c\<^bold>o\<^bold>n\<^bold>v Merge P (N \<heavy_comma> R) (1 \<heavy_comma> \<blangle> L \<heavy_comma> OBJ H1\<brangle>) = X \<^bold>@\<^bold>G\<^bold>O\<^bold>A\<^bold>L G
+   \<Longrightarrow> \<^bold>c\<^bold>o\<^bold>n\<^bold>v Merge (MergeNeg P) (L \<heavy_comma> OBJ H1) (N \<heavy_comma> \<blangle> R \<brangle>) = X \<^bold>@\<^bold>G\<^bold>O\<^bold>A\<^bold>L G"
   unfolding Conv_def cast_def Merge_def MergeNeg_def by force
 
-lemma (in std) [\<phi>reason 100 on \<open>\<medium_left_bracket> \<^bold>c\<^bold>o\<^bold>n\<^bold>v Merge ?P (?L \<heavy_comma> OBJ ?H1) (?N \<heavy_comma> \<medium_left_bracket> ?R \<heavy_comma> OBJ ?H2 \<medium_right_bracket>) = ?X''' \<medium_right_bracket>: ?G\<close>]:
+lemma (in std) [\<phi>reason 100 on \<open>\<^bold>c\<^bold>o\<^bold>n\<^bold>v Merge ?P (?L \<heavy_comma> OBJ ?H1) (?N \<heavy_comma> \<blangle> ?R \<heavy_comma> OBJ ?H2 \<brangle>) = ?X''' \<^bold>@\<^bold>G\<^bold>O\<^bold>A\<^bold>L ?G\<close>]:
   \<comment> \<open>search the immediate element\<close>
   "CHK_SUBGOAL G
    \<Longrightarrow> EqualAddress H1 H2
    \<Longrightarrow> \<^bold>c\<^bold>o\<^bold>n\<^bold>v Merge P (OBJ H1) (OBJ H2) = H
    \<Longrightarrow> SOLVE_SUBGOAL G \<comment> \<open>if success, trim all other branches on G\<close>
    \<Longrightarrow> SUBGOAL G G2
-   \<Longrightarrow> \<medium_left_bracket> \<^bold>c\<^bold>o\<^bold>n\<^bold>v Merge P L (1 \<heavy_comma> \<medium_left_bracket> N \<heavy_comma> R \<medium_right_bracket>) = X \<medium_right_bracket>: G2
-   \<Longrightarrow> \<medium_left_bracket> \<^bold>c\<^bold>o\<^bold>n\<^bold>v Merge P (L \<heavy_comma> OBJ H1) (N \<heavy_comma> \<medium_left_bracket> R \<heavy_comma> OBJ H2 \<medium_right_bracket>) = (X \<heavy_comma> H) \<medium_right_bracket>: G"
+   \<Longrightarrow> \<^bold>c\<^bold>o\<^bold>n\<^bold>v Merge P L (1 \<heavy_comma> \<blangle> N \<heavy_comma> R \<brangle>) = X \<^bold>@\<^bold>G\<^bold>O\<^bold>A\<^bold>L G2
+   \<Longrightarrow> \<^bold>c\<^bold>o\<^bold>n\<^bold>v Merge P (L \<heavy_comma> OBJ H1) (N \<heavy_comma> \<blangle> R \<heavy_comma> OBJ H2 \<brangle>) = (X \<heavy_comma> H) \<^bold>@\<^bold>G\<^bold>O\<^bold>A\<^bold>L G"
   unfolding Conv_def cast_def Merge_def mult_1_left by (metis mult.assoc)
 
-lemma (in std) [\<phi>reason 70 on \<open>\<medium_left_bracket> \<^bold>c\<^bold>o\<^bold>n\<^bold>v Merge ?P ?L (?N \<heavy_comma> \<medium_left_bracket> ?R \<heavy_comma> OBJ ?H2 \<medium_right_bracket>) = ?X''' \<medium_right_bracket>: ?G\<close>]:
+lemma (in std) [\<phi>reason 70 on \<open>\<^bold>c\<^bold>o\<^bold>n\<^bold>v Merge ?P ?L (?N \<heavy_comma> \<blangle> ?R \<heavy_comma> OBJ ?H2 \<brangle>) = ?X''' \<^bold>@\<^bold>G\<^bold>O\<^bold>A\<^bold>L ?G\<close>]:
   \<comment> \<open>search next\<close>
   "CHK_SUBGOAL G
-   \<Longrightarrow> \<medium_left_bracket> \<^bold>c\<^bold>o\<^bold>n\<^bold>v Merge P L (N \<heavy_comma> OBJ H2 \<heavy_comma> \<medium_left_bracket> R \<medium_right_bracket>) = X \<medium_right_bracket>: G
-   \<Longrightarrow> \<medium_left_bracket> \<^bold>c\<^bold>o\<^bold>n\<^bold>v Merge P L (N \<heavy_comma> \<medium_left_bracket> R \<heavy_comma> OBJ H2 \<medium_right_bracket>) = X \<medium_right_bracket>: G"
+   \<Longrightarrow> \<^bold>c\<^bold>o\<^bold>n\<^bold>v Merge P L (N \<heavy_comma> OBJ H2 \<heavy_comma> \<blangle> R \<brangle>) = X \<^bold>@\<^bold>G\<^bold>O\<^bold>A\<^bold>L G
+   \<Longrightarrow> \<^bold>c\<^bold>o\<^bold>n\<^bold>v Merge P L (N \<heavy_comma> \<blangle> R \<heavy_comma> OBJ H2 \<brangle>) = X \<^bold>@\<^bold>G\<^bold>O\<^bold>A\<^bold>L G"
   unfolding Conv_def cast_def by (metis mult.assoc OBJ_comm)
 
 subsubsection \<open>Unfold\<close>
 
 lemma (in std) [\<phi>reason 2000]:
-  "\<medium_left_bracket> \<^bold>c\<^bold>o\<^bold>n\<^bold>v Merge P L (N \<heavy_comma> \<medium_left_bracket> R \<heavy_comma> R1 \<heavy_comma> R2 \<medium_right_bracket>) = X \<medium_right_bracket>: G
-   \<Longrightarrow> \<medium_left_bracket> \<^bold>c\<^bold>o\<^bold>n\<^bold>v Merge P L (N \<heavy_comma> \<medium_left_bracket> R \<heavy_comma> (R1 \<heavy_comma> R2) \<medium_right_bracket>) = X \<medium_right_bracket>: G"
+  "\<^bold>c\<^bold>o\<^bold>n\<^bold>v Merge P L (N \<heavy_comma> \<blangle> R \<heavy_comma> R1 \<heavy_comma> R2 \<brangle>) = X \<^bold>@\<^bold>G\<^bold>O\<^bold>A\<^bold>L G
+   \<Longrightarrow> \<^bold>c\<^bold>o\<^bold>n\<^bold>v Merge P L (N \<heavy_comma> \<blangle> R \<heavy_comma> (R1 \<heavy_comma> R2) \<brangle>) = X \<^bold>@\<^bold>G\<^bold>O\<^bold>A\<^bold>L G"
   unfolding Conv_def cast_def by (metis mult.assoc)
 
 lemma (in std) [\<phi>reason 2000]:
-  "\<medium_left_bracket> \<^bold>c\<^bold>o\<^bold>n\<^bold>v Merge P (L1 \<heavy_comma> L2 \<heavy_comma> L3) R = X \<medium_right_bracket>: G
-   \<Longrightarrow> \<medium_left_bracket> \<^bold>c\<^bold>o\<^bold>n\<^bold>v Merge P (L1 \<heavy_comma> (L2 \<heavy_comma> L3)) R = X \<medium_right_bracket>: G"
+  "\<^bold>c\<^bold>o\<^bold>n\<^bold>v Merge P (L1 \<heavy_comma> L2 \<heavy_comma> L3) R = X \<^bold>@\<^bold>G\<^bold>O\<^bold>A\<^bold>L G
+   \<Longrightarrow> \<^bold>c\<^bold>o\<^bold>n\<^bold>v Merge P (L1 \<heavy_comma> (L2 \<heavy_comma> L3)) R = X \<^bold>@\<^bold>G\<^bold>O\<^bold>A\<^bold>L G"
   unfolding Conv_def cast_def by (metis mult.assoc)
 
 lemma (in std) [\<phi>reason 2200]:
-  "\<medium_left_bracket> \<^bold>c\<^bold>o\<^bold>n\<^bold>v Merge P L (N \<heavy_comma> \<medium_left_bracket> R1 \<heavy_comma> R2 \<medium_right_bracket>) = X \<medium_right_bracket>: G
-   \<Longrightarrow> \<medium_left_bracket> \<^bold>c\<^bold>o\<^bold>n\<^bold>v Merge P L (N \<heavy_comma> \<medium_left_bracket> 1 \<heavy_comma> (R1 \<heavy_comma> R2) \<medium_right_bracket>) = X \<medium_right_bracket>: G"
+  "\<^bold>c\<^bold>o\<^bold>n\<^bold>v Merge P L (N \<heavy_comma> \<blangle> R1 \<heavy_comma> R2 \<brangle>) = X \<^bold>@\<^bold>G\<^bold>O\<^bold>A\<^bold>L G
+   \<Longrightarrow> \<^bold>c\<^bold>o\<^bold>n\<^bold>v Merge P L (N \<heavy_comma> \<blangle> 1 \<heavy_comma> (R1 \<heavy_comma> R2) \<brangle>) = X \<^bold>@\<^bold>G\<^bold>O\<^bold>A\<^bold>L G"
   unfolding Conv_def cast_def by force
 
 
 subsubsection \<open>Padding 1\<close>
 
 lemma (in std) [\<phi>reason 2000]:
-  "\<medium_left_bracket> \<^bold>c\<^bold>o\<^bold>n\<^bold>v Merge P (1 \<heavy_comma> OBJ L) R = X \<medium_right_bracket>: G
-   \<Longrightarrow> \<medium_left_bracket> \<^bold>c\<^bold>o\<^bold>n\<^bold>v Merge P (OBJ L) R = X \<medium_right_bracket>: G"
+  "\<^bold>c\<^bold>o\<^bold>n\<^bold>v Merge P (1 \<heavy_comma> OBJ L) R = X \<^bold>@\<^bold>G\<^bold>O\<^bold>A\<^bold>L G
+   \<Longrightarrow> \<^bold>c\<^bold>o\<^bold>n\<^bold>v Merge P (OBJ L) R = X \<^bold>@\<^bold>G\<^bold>O\<^bold>A\<^bold>L G"
   unfolding Conv_def cast_def by force
 
 lemma (in std) [\<phi>reason 2000]:
-  "\<medium_left_bracket> \<^bold>c\<^bold>o\<^bold>n\<^bold>v Merge P (1 \<heavy_comma> VAL L) R = X \<medium_right_bracket>: G
-   \<Longrightarrow> \<medium_left_bracket> \<^bold>c\<^bold>o\<^bold>n\<^bold>v Merge P (VAL L) R = X \<medium_right_bracket>: G"
+  "\<^bold>c\<^bold>o\<^bold>n\<^bold>v Merge P (1 \<heavy_comma> VAL L) R = X \<^bold>@\<^bold>G\<^bold>O\<^bold>A\<^bold>L G
+   \<Longrightarrow> \<^bold>c\<^bold>o\<^bold>n\<^bold>v Merge P (VAL L) R = X \<^bold>@\<^bold>G\<^bold>O\<^bold>A\<^bold>L G"
   unfolding Conv_def cast_def by force
 
 lemma (in std) [\<phi>reason 2000]:
-  "\<medium_left_bracket> \<^bold>c\<^bold>o\<^bold>n\<^bold>v Merge P L (N \<heavy_comma> \<medium_left_bracket> 1 \<heavy_comma> VAL V \<medium_right_bracket>) = X \<medium_right_bracket>: G
-   \<Longrightarrow> \<medium_left_bracket> \<^bold>c\<^bold>o\<^bold>n\<^bold>v Merge P L (N \<heavy_comma> \<medium_left_bracket> VAL V \<medium_right_bracket>) = X \<medium_right_bracket>: G"
+  "\<^bold>c\<^bold>o\<^bold>n\<^bold>v Merge P L (N \<heavy_comma> \<blangle> 1 \<heavy_comma> VAL V \<brangle>) = X \<^bold>@\<^bold>G\<^bold>O\<^bold>A\<^bold>L G
+   \<Longrightarrow> \<^bold>c\<^bold>o\<^bold>n\<^bold>v Merge P L (N \<heavy_comma> \<blangle> VAL V \<brangle>) = X \<^bold>@\<^bold>G\<^bold>O\<^bold>A\<^bold>L G"
   unfolding Conv_def cast_def by force
 
 lemma (in std) [\<phi>reason 2000]:
-  "\<medium_left_bracket> \<^bold>c\<^bold>o\<^bold>n\<^bold>v Merge P L (N \<heavy_comma> \<medium_left_bracket> 1 \<heavy_comma> OBJ V \<medium_right_bracket>) = X \<medium_right_bracket>: G
-   \<Longrightarrow> \<medium_left_bracket> \<^bold>c\<^bold>o\<^bold>n\<^bold>v Merge P L (N \<heavy_comma> \<medium_left_bracket> OBJ V \<medium_right_bracket>) = X \<medium_right_bracket>: G"
+  "\<^bold>c\<^bold>o\<^bold>n\<^bold>v Merge P L (N \<heavy_comma> \<blangle> 1 \<heavy_comma> OBJ V \<brangle>) = X \<^bold>@\<^bold>G\<^bold>O\<^bold>A\<^bold>L G
+   \<Longrightarrow> \<^bold>c\<^bold>o\<^bold>n\<^bold>v Merge P L (N \<heavy_comma> \<blangle> OBJ V \<brangle>) = X \<^bold>@\<^bold>G\<^bold>O\<^bold>A\<^bold>L G"
   unfolding Conv_def cast_def by force
 
 subsubsection \<open>Eliminate 1 Hole\<close>
 
 lemma (in std) [\<phi>reason 2000]:
-  "\<medium_left_bracket> \<^bold>c\<^bold>o\<^bold>n\<^bold>v Merge P L (N \<heavy_comma> \<medium_left_bracket> R \<medium_right_bracket>) = X \<medium_right_bracket>: G
-   \<Longrightarrow> \<medium_left_bracket> \<^bold>c\<^bold>o\<^bold>n\<^bold>v Merge P L (N \<heavy_comma> \<medium_left_bracket> R \<heavy_comma> 1 \<medium_right_bracket>) = X \<medium_right_bracket>: G"
+  "\<^bold>c\<^bold>o\<^bold>n\<^bold>v Merge P L (N \<heavy_comma> \<blangle> R \<brangle>) = X \<^bold>@\<^bold>G\<^bold>O\<^bold>A\<^bold>L G
+   \<Longrightarrow> \<^bold>c\<^bold>o\<^bold>n\<^bold>v Merge P L (N \<heavy_comma> \<blangle> R \<heavy_comma> 1 \<brangle>) = X \<^bold>@\<^bold>G\<^bold>O\<^bold>A\<^bold>L G"
   unfolding Conv_def cast_def by force
 
 lemma (in std) [\<phi>reason 2000]:
-  "\<medium_left_bracket> \<^bold>c\<^bold>o\<^bold>n\<^bold>v Merge P L R = X \<medium_right_bracket>: G
-   \<Longrightarrow> \<medium_left_bracket> \<^bold>c\<^bold>o\<^bold>n\<^bold>v Merge P (L \<heavy_comma> 1) R = X \<medium_right_bracket>: G"
+  "\<^bold>c\<^bold>o\<^bold>n\<^bold>v Merge P L R = X \<^bold>@\<^bold>G\<^bold>O\<^bold>A\<^bold>L G
+   \<Longrightarrow> \<^bold>c\<^bold>o\<^bold>n\<^bold>v Merge P (L \<heavy_comma> 1) R = X \<^bold>@\<^bold>G\<^bold>O\<^bold>A\<^bold>L G"
   unfolding Conv_def cast_def by force
 
 subsubsection \<open>Termination\<close>
 
-lemma (in std) [\<phi>reason 2000 on \<open>\<medium_left_bracket> \<^bold>c\<^bold>o\<^bold>n\<^bold>v Merge ?P 1 (1 \<heavy_comma> \<medium_left_bracket> 1 \<medium_right_bracket>) = ?X'' \<medium_right_bracket>: ?G\<close>]:
-  "\<medium_left_bracket> \<^bold>c\<^bold>o\<^bold>n\<^bold>v Merge P 1 (1 \<heavy_comma> \<medium_left_bracket> 1 \<medium_right_bracket>) = 1 \<medium_right_bracket>: G"
+lemma (in std) [\<phi>reason 2000 on \<open>\<^bold>c\<^bold>o\<^bold>n\<^bold>v Merge ?P 1 (1 \<heavy_comma> \<blangle> 1 \<brangle>) = ?X'' \<^bold>@\<^bold>G\<^bold>O\<^bold>A\<^bold>L ?G\<close>]:
+  "\<^bold>c\<^bold>o\<^bold>n\<^bold>v Merge P 1 (1 \<heavy_comma> \<blangle> 1 \<brangle>) = 1 \<^bold>@\<^bold>G\<^bold>O\<^bold>A\<^bold>L G"
   unfolding Conv_def cast_def Merge_def by force
   
 
@@ -2223,20 +2264,19 @@ val structured_statement =
   nustatement -- Parse_Spec.if_statement' -- Parse.for_fixes
     >> (fn ((shows, assumes), fixes) => (fixes, assumes, shows));
 val statement1 = Parse.and_list1 (Parse_Spec.opt_thm_name ":" -- Parse.propp);
-val requires_statement = $$$ "requires" |-- Parse.!!! statement1;
-val premises_statement = $$$ "premises" |-- Parse.!!! statement1;
+val requires_statement = \<^keyword>\<open>assumes\<close> |-- Parse.!!! statement1;
+val premises_statement = \<^keyword>\<open>premises\<close> |-- Parse.!!! statement1;
 val precond_statement = Scan.repeat ((premises_statement >> map (pair NuToplevel.Premise))
                 || (requires_statement >> map (pair NuToplevel.Requirement))) >> flat;
-val requires_opt1 = Scan.option ($$$ "requires" |-- Parse.term);
-val where_statement = Scan.optional ($$$ "where" |--
+val requires_opt1 = Scan.option (\<^keyword>\<open>assumes\<close> |-- Parse.term);
+val where_statement = Scan.optional (\<^keyword>\<open>where\<close> |--
         Parse.and_list1 (Scan.repeat Args.var --| Parse.$$$ "=" -- Parse.term)) [];
 val defines_statement = Scan.optional ($$$ "defines" |-- Parse.!!! statement1) [];
 val nu_statements = Parse.for_fixes -- Scan.optional Parse_Spec.includes [] --
            where_statement -- defines_statement  -- precond_statement;
 
 val arg = Parse.term
-val proc_head = Parse_Spec.thm_name ":" --
-        ((arg --| $$$ "\<longmapsto>" -- arg) || ($$$ "argument" |-- arg --| $$$ "return" -- arg))
+val arg_ret = (\<^keyword>\<open>argument\<close> |-- arg --| \<^keyword>\<open>return\<close> -- arg)
 
 in
 
@@ -2245,22 +2285,22 @@ in
 
 val _ =
   Outer_Syntax.local_theory_to_proof' \<^command_keyword>\<open>proc\<close> "begin a procedure construction"
-    ((proc_head -- nu_statements) >>
-        (fn ((b,(arg,ret)),((((fixes,includes),lets),defs),preconds)) =>  
+    ((Parse_Spec.thm_name ":" -- nu_statements -- arg_ret) >>
+        (fn ((b,((((fixes,includes),lets),defs),preconds)), (arg,ret)) =>  
             (begin_proc_cmd b arg ret fixes includes lets defs preconds)));
 
 val loop_variables = $$$ "var" |-- !!! vars;
 val _ =
   Outer_Syntax.local_theory_to_proof' \<^command_keyword>\<open>rec_proc\<close> "begin a recursive procedure construction"
-    ((proc_head -- loop_variables -- nu_statements) >>
-        (fn (((b,(arg,ret)),vars),((((fixes,includes),lets),defs),preconds)) =>  
+    ((Parse_Spec.thm_name ":" -- loop_variables -- nu_statements -- arg_ret) >>
+        (fn (((b,vars),((((fixes,includes),lets),defs),preconds)), (arg,ret)) =>  
             (begin_rec_proc_cmd b arg ret (vars,fixes) includes lets defs preconds)));
 
-val _ =
+(* val _ =
   Outer_Syntax.local_theory_to_proof' \<^command_keyword>\<open>\<phi>cast\<close> "begin a procedure construction"
-    ((proc_head -- option ($$$ "and" |-- Parse.term) -- nu_statements) >>
-        (fn (((b,(arg,ret)),addtional_prop),((((fixes,includes),lets),defs),preconds)) =>
-            (begin_cast_cmd b arg ret addtional_prop fixes includes lets defs preconds)));
+    ((Parse_Spec.thm_name ":" -- option ($$$ "and" |-- Parse.term) -- nu_statements - arg_ret) >>
+        (fn ((b,((((fixes,includes),lets),defs),preconds)), (arg,ret)) =>
+            (begin_cast_cmd b arg ret fixes includes lets defs preconds))); *)
 
 val _ =
   Outer_Syntax.command \<^command_keyword>\<open>;;\<close> "Lead statements of \<phi> programs"
@@ -2350,11 +2390,14 @@ subsubsection \<open>Constructive\<close>
          of SOME (th, _) => (ctxt,th)
           | _ => raise THM ("RSN: no unifiers", 1, sequent::apps) end)\<close>
 
+ML \<open>val phi_synthesis_parsing = Config.declare_bool ("\<phi>_synthesis_parsing", \<^here>) (K false)\<close>
+
 \<phi>processor synthesis 8000 (\<open>\<^bold>c\<^bold>u\<^bold>r\<^bold>r\<^bold>e\<^bold>n\<^bold>t ?blk [?H] \<^bold>r\<^bold>e\<^bold>s\<^bold>u\<^bold>l\<^bold>t\<^bold>s \<^bold>i\<^bold>n ?S\<close>)
   \<open>fn (ctxt, sequent) => Parse.group (fn () => "term") (Parse.inner_syntax (Parse.cartouche || Parse.number))
 >> (fn raw_term => fn () =>
   let
     val ctxt_parser = Proof_Context.set_mode Proof_Context.mode_pattern ctxt
+                        |> Config.put phi_synthesis_parsing true
     fun add_ele tm = Const (\<^const_name>\<open>Ele\<close>, dummyT) $ tm
     fun chk_term' (\<^typ>\<open>('VAL,'FIC_N,'FIC) assn\<close>) tm = tm
       | chk_term' _ (tm as (Const (\<^const_name>\<open>\<phi>Type\<close>, _) $ _ $ _)) = add_ele tm
