NuLLReps.thy
@@ -469,40 +469,41 @@ lemma Var_SubjTyp[simp]:
   \<open>(x \<Ztypecolon> Var vname (T \<phi>\<^bold>s\<^bold>u\<^bold>b\<^bold>j P)) = (x \<Ztypecolon> Var vname T \<^bold>s\<^bold>u\<^bold>b\<^bold>j P)\<close>
   unfolding set_eq_iff by (simp add: \<phi>expns, blast)
 
-lemma [\<phi>reason 110 on \<open>\<medium_left_bracket> \<^bold>s\<^bold>u\<^bold>b\<^bold>t\<^bold>y\<^bold>p\<^bold>e ?R \<heavy_comma> OBJ ?H \<longmapsto> ?R''' * \<medium_left_bracket> OBJ ?X \<medium_right_bracket> \<^bold>w\<^bold>i\<^bold>t\<^bold>h ?P \<medium_right_bracket>: ?G\<close>]: \<comment> \<open>attempts the immediate cell\<close>
+lemma [\<phi>reason 110 on \<open>\<^bold>s\<^bold>u\<^bold>b\<^bold>t\<^bold>y\<^bold>p\<^bold>e ?R \<heavy_comma> OBJ ?H \<longmapsto> ?R''' * \<blangle> OBJ ?X \<brangle> \<^bold>w\<^bold>i\<^bold>t\<^bold>h ?P \<^bold>@\<^bold>G\<^bold>O\<^bold>A\<^bold>L ?G\<close>]: \<comment> \<open>attempts the immediate cell\<close>
   " CHK_SUBGOAL G
 \<Longrightarrow> \<^bold>s\<^bold>u\<^bold>b\<^bold>t\<^bold>y\<^bold>p\<^bold>e x \<Ztypecolon> T \<longmapsto> x' \<Ztypecolon> T' \<^bold>w\<^bold>i\<^bold>t\<^bold>h P
-\<Longrightarrow> \<medium_left_bracket> \<^bold>s\<^bold>u\<^bold>b\<^bold>t\<^bold>y\<^bold>p\<^bold>e R\<heavy_comma> OBJ x \<Ztypecolon> Var var T \<longmapsto> R\<heavy_comma> \<medium_left_bracket> OBJ x' \<Ztypecolon> Var var T' \<medium_right_bracket> \<^bold>w\<^bold>i\<^bold>t\<^bold>h P \<medium_right_bracket>: G"
+\<Longrightarrow> \<^bold>s\<^bold>u\<^bold>b\<^bold>t\<^bold>y\<^bold>p\<^bold>e R\<heavy_comma> OBJ x \<Ztypecolon> Var var T \<longmapsto> R\<heavy_comma> \<blangle> OBJ x' \<Ztypecolon> Var var T' \<brangle> \<^bold>w\<^bold>i\<^bold>t\<^bold>h P \<^bold>@\<^bold>G\<^bold>O\<^bold>A\<^bold>L G"
   unfolding cast_def
   by (simp add: \<phi>expns times_list_def, blast)
 
 
 subsubsection \<open>Synthesis Rules\<close>
 
-lemma [\<phi>reason on \<open>\<medium_left_bracket> \<^bold>p\<^bold>r\<^bold>o\<^bold>c ?f \<lbrace> ?S1 \<longmapsto> ?S2\<heavy_comma> SYNTHESIS ?x \<Ztypecolon> Var ?var ?T \<rbrace> \<medium_right_bracket>: ?G\<close>]:
+lemma [\<phi>reason on \<open>\<^bold>p\<^bold>r\<^bold>o\<^bold>c ?f \<lbrace> ?S1 \<longmapsto> ?S2\<heavy_comma> SYNTHESIS ?x \<Ztypecolon> Var ?var ?T \<rbrace> \<^bold>@\<^bold>G\<^bold>O\<^bold>A\<^bold>L ?G\<close>]:
   \<open> SUBGOAL G G'
-\<Longrightarrow> \<medium_left_bracket> \<^bold>s\<^bold>u\<^bold>b\<^bold>t\<^bold>y\<^bold>p\<^bold>e S1 \<longmapsto> S2\<heavy_comma> \<medium_left_bracket> OBJ x \<Ztypecolon> Var var T \<medium_right_bracket> \<medium_right_bracket>: G'
+\<Longrightarrow> \<^bold>s\<^bold>u\<^bold>b\<^bold>t\<^bold>y\<^bold>p\<^bold>e S1 \<longmapsto> S2\<heavy_comma> \<blangle> OBJ x \<Ztypecolon> Var var T \<brangle> \<^bold>@\<^bold>G\<^bold>O\<^bold>A\<^bold>L G'
 \<Longrightarrow> SOLVE_SUBGOAL G'
-\<Longrightarrow> \<medium_left_bracket> \<^bold>p\<^bold>r\<^bold>o\<^bold>c SKIP \<lbrace> S1 \<longmapsto> S2\<heavy_comma> SYNTHESIS x \<Ztypecolon> Var var T \<rbrace> \<medium_right_bracket>: G\<close>
-  unfolding Subty_Target2_def Subty_Target_def Synthesis_def
-  using "\<phi>cast" \<phi>reassemble_proc_0 \<phi>reassemble_proc_final by blast
+\<Longrightarrow> \<^bold>p\<^bold>r\<^bold>o\<^bold>c SKIP \<lbrace> S1 \<longmapsto> S2\<heavy_comma> SYNTHESIS x \<Ztypecolon> Var var T \<rbrace> \<^bold>@\<^bold>G\<^bold>O\<^bold>A\<^bold>L G\<close>
+  unfolding GOAL_CTXT_def FOCUS_TAG_def Synthesis_def
+  using "\<phi>cast" \<phi>reassemble_proc_0 \<phi>reassemble_proc_final
+  by (metis EMPTY_PROC_def)
 
 
 subsubsection \<open>Application Methods for Subtyping\<close>
 
 lemma [\<phi>reason 2000 on \<open>
-  PROP \<phi>Application_Method (\<^bold>s\<^bold>u\<^bold>b\<^bold>t\<^bold>y\<^bold>p\<^bold>e ?x \<Ztypecolon> ?T \<longmapsto> ?Y \<Ztypecolon> ?U \<^bold>w\<^bold>i\<^bold>t\<^bold>h ?P)
+  PROP \<phi>Application_Method (Trueprop (\<^bold>s\<^bold>u\<^bold>b\<^bold>t\<^bold>y\<^bold>p\<^bold>e ?x \<Ztypecolon> ?T \<longmapsto> ?Y \<Ztypecolon> ?U \<^bold>w\<^bold>i\<^bold>t\<^bold>h ?P))
             (\<^bold>c\<^bold>u\<^bold>r\<^bold>r\<^bold>e\<^bold>n\<^bold>t ?blk [?RR] \<^bold>r\<^bold>e\<^bold>s\<^bold>u\<^bold>l\<^bold>t\<^bold>s \<^bold>i\<^bold>n OBJ ?x \<Ztypecolon> Var ?var ?T) ?Result
 \<close>]:
   \<open> PROP \<phi>Application_Success
-\<Longrightarrow> PROP \<phi>Application_Method (\<^bold>s\<^bold>u\<^bold>b\<^bold>t\<^bold>y\<^bold>p\<^bold>e x \<Ztypecolon> T \<longmapsto> x \<Ztypecolon> U \<^bold>w\<^bold>i\<^bold>t\<^bold>h P)
+\<Longrightarrow> PROP \<phi>Application_Method (Trueprop (\<^bold>s\<^bold>u\<^bold>b\<^bold>t\<^bold>y\<^bold>p\<^bold>e x \<Ztypecolon> T \<longmapsto> x \<Ztypecolon> U \<^bold>w\<^bold>i\<^bold>t\<^bold>h P))
       (\<^bold>c\<^bold>u\<^bold>r\<^bold>r\<^bold>e\<^bold>n\<^bold>t blk [RR] \<^bold>r\<^bold>e\<^bold>s\<^bold>u\<^bold>l\<^bold>t\<^bold>s \<^bold>i\<^bold>n OBJ x \<Ztypecolon> Var var T)
       (Trueprop ((\<^bold>c\<^bold>u\<^bold>r\<^bold>r\<^bold>e\<^bold>n\<^bold>t blk [RR] \<^bold>r\<^bold>e\<^bold>s\<^bold>u\<^bold>l\<^bold>t\<^bold>s \<^bold>i\<^bold>n OBJ x \<Ztypecolon> Var var U) \<and> P))\<close>
   unfolding \<phi>Application_Method_def \<phi>Application_def
   using "\<phi>cast_P" Var_cast_\<phi>app[unfolded Argument_def Fix_def] by metis
 
 lemma [\<phi>reason 2000 on \<open>
-  PROP \<phi>Application_Method (\<^bold>s\<^bold>u\<^bold>b\<^bold>t\<^bold>y\<^bold>p\<^bold>e ?x' \<Ztypecolon> ?T' \<longmapsto> ?y \<Ztypecolon> ?U \<^bold>w\<^bold>i\<^bold>t\<^bold>h ?P)
+  PROP \<phi>Application_Method (Trueprop (\<^bold>s\<^bold>u\<^bold>b\<^bold>t\<^bold>y\<^bold>p\<^bold>e ?x' \<Ztypecolon> ?T' \<longmapsto> ?y \<Ztypecolon> ?U \<^bold>w\<^bold>i\<^bold>t\<^bold>h ?P))
             (\<^bold>c\<^bold>u\<^bold>r\<^bold>r\<^bold>e\<^bold>n\<^bold>t ?blk [?RR] \<^bold>r\<^bold>e\<^bold>s\<^bold>u\<^bold>l\<^bold>t\<^bold>s \<^bold>i\<^bold>n OBJ ?x \<Ztypecolon> Var ?var ?T) ?Result
 \<close>]:
   \<open> SUBGOAL TOP_GOAL G
@@ -510,7 +511,7 @@ lemma [\<phi>reason 2000 on \<open>
 \<Longrightarrow> SOLVE_SUBGOAL G
 \<Longrightarrow> PROP \<phi>Application_Success
 \<Longrightarrow> \<^bold>o\<^bold>b\<^bold>l\<^bold>i\<^bold>g\<^bold>a\<^bold>t\<^bold>i\<^bold>o\<^bold>n True
-\<Longrightarrow> PROP \<phi>Application_Method (\<^bold>s\<^bold>u\<^bold>b\<^bold>t\<^bold>y\<^bold>p\<^bold>e x' \<Ztypecolon> T' \<longmapsto> y \<Ztypecolon> U \<^bold>w\<^bold>i\<^bold>t\<^bold>h P)
+\<Longrightarrow> PROP \<phi>Application_Method (Trueprop (\<^bold>s\<^bold>u\<^bold>b\<^bold>t\<^bold>y\<^bold>p\<^bold>e x' \<Ztypecolon> T' \<longmapsto> y \<Ztypecolon> U \<^bold>w\<^bold>i\<^bold>t\<^bold>h P))
       (\<^bold>c\<^bold>u\<^bold>r\<^bold>r\<^bold>e\<^bold>n\<^bold>t blk [RR] \<^bold>r\<^bold>e\<^bold>s\<^bold>u\<^bold>l\<^bold>t\<^bold>s \<^bold>i\<^bold>n OBJ x \<Ztypecolon> Var var T)
       (Trueprop ((\<^bold>c\<^bold>u\<^bold>r\<^bold>r\<^bold>e\<^bold>n\<^bold>t blk [RR] \<^bold>r\<^bold>e\<^bold>s\<^bold>u\<^bold>l\<^bold>t\<^bold>s \<^bold>i\<^bold>n OBJ y \<Ztypecolon> Var var U) \<and> P))\<close>
   unfolding \<phi>Application_Method_def \<phi>Application_def
@@ -518,11 +519,11 @@ lemma [\<phi>reason 2000 on \<open>
 
 
 lemma [\<phi>reason 2000 on \<open>
-  PROP \<phi>Application_Method (\<^bold>s\<^bold>u\<^bold>b\<^bold>t\<^bold>y\<^bold>p\<^bold>e ?x \<Ztypecolon> ?T \<longmapsto> ?y \<Ztypecolon> ?U \<^bold>w\<^bold>i\<^bold>t\<^bold>h ?P)
+  PROP \<phi>Application_Method (Trueprop (\<^bold>s\<^bold>u\<^bold>b\<^bold>t\<^bold>y\<^bold>p\<^bold>e ?x \<Ztypecolon> ?T \<longmapsto> ?y \<Ztypecolon> ?U \<^bold>w\<^bold>i\<^bold>t\<^bold>h ?P))
           (\<^bold>c\<^bold>u\<^bold>r\<^bold>r\<^bold>e\<^bold>n\<^bold>t ?blk [?RR] \<^bold>r\<^bold>e\<^bold>s\<^bold>u\<^bold>l\<^bold>t\<^bold>s \<^bold>i\<^bold>n ?R\<heavy_comma> OBJ ?x \<Ztypecolon> Var ?var ?T) ?Result
 \<close>]:
   \<open> PROP \<phi>Application_Success
-\<Longrightarrow> PROP \<phi>Application_Method (\<^bold>s\<^bold>u\<^bold>b\<^bold>t\<^bold>y\<^bold>p\<^bold>e x \<Ztypecolon> T \<longmapsto> y \<Ztypecolon> U \<^bold>w\<^bold>i\<^bold>t\<^bold>h P)
+\<Longrightarrow> PROP \<phi>Application_Method (Trueprop (\<^bold>s\<^bold>u\<^bold>b\<^bold>t\<^bold>y\<^bold>p\<^bold>e x \<Ztypecolon> T \<longmapsto> y \<Ztypecolon> U \<^bold>w\<^bold>i\<^bold>t\<^bold>h P))
       (\<^bold>c\<^bold>u\<^bold>r\<^bold>r\<^bold>e\<^bold>n\<^bold>t blk [RR] \<^bold>r\<^bold>e\<^bold>s\<^bold>u\<^bold>l\<^bold>t\<^bold>s \<^bold>i\<^bold>n R\<heavy_comma> OBJ x \<Ztypecolon> Var var T)
       (Trueprop ((\<^bold>c\<^bold>u\<^bold>r\<^bold>r\<^bold>e\<^bold>n\<^bold>t blk [RR] \<^bold>r\<^bold>e\<^bold>s\<^bold>u\<^bold>l\<^bold>t\<^bold>s \<^bold>i\<^bold>n R\<heavy_comma> OBJ y \<Ztypecolon> Var var U) \<and> P))\<close>
   unfolding \<phi>Application_Method_def \<phi>Application_def
@@ -530,7 +531,7 @@ lemma [\<phi>reason 2000 on \<open>
 
 
 lemma [\<phi>reason 2000 on \<open>
-  PROP \<phi>Application_Method (\<^bold>s\<^bold>u\<^bold>b\<^bold>t\<^bold>y\<^bold>p\<^bold>e ?x' \<Ztypecolon> ?T' \<longmapsto> ?y \<Ztypecolon> ?U \<^bold>w\<^bold>i\<^bold>t\<^bold>h ?P)
+  PROP \<phi>Application_Method (Trueprop (\<^bold>s\<^bold>u\<^bold>b\<^bold>t\<^bold>y\<^bold>p\<^bold>e ?x' \<Ztypecolon> ?T' \<longmapsto> ?y \<Ztypecolon> ?U \<^bold>w\<^bold>i\<^bold>t\<^bold>h ?P))
       (\<^bold>c\<^bold>u\<^bold>r\<^bold>r\<^bold>e\<^bold>n\<^bold>t ?blk [?RR] \<^bold>r\<^bold>e\<^bold>s\<^bold>u\<^bold>l\<^bold>t\<^bold>s \<^bold>i\<^bold>n ?R\<heavy_comma> OBJ ?x \<Ztypecolon> Var ?var ?T) ?Result
 \<close>]:
   \<open> SUBGOAL TOP_GOAL G
@@ -538,7 +539,7 @@ lemma [\<phi>reason 2000 on \<open>
 \<Longrightarrow> SOLVE_SUBGOAL G
 \<Longrightarrow> PROP \<phi>Application_Success
 \<Longrightarrow> \<^bold>o\<^bold>b\<^bold>l\<^bold>i\<^bold>g\<^bold>a\<^bold>t\<^bold>i\<^bold>o\<^bold>n True
-\<Longrightarrow> PROP \<phi>Application_Method (\<^bold>s\<^bold>u\<^bold>b\<^bold>t\<^bold>y\<^bold>p\<^bold>e x' \<Ztypecolon> T' \<longmapsto> y \<Ztypecolon> U \<^bold>w\<^bold>i\<^bold>t\<^bold>h P)
+\<Longrightarrow> PROP \<phi>Application_Method (Trueprop (\<^bold>s\<^bold>u\<^bold>b\<^bold>t\<^bold>y\<^bold>p\<^bold>e x' \<Ztypecolon> T' \<longmapsto> y \<Ztypecolon> U \<^bold>w\<^bold>i\<^bold>t\<^bold>h P))
       (\<^bold>c\<^bold>u\<^bold>r\<^bold>r\<^bold>e\<^bold>n\<^bold>t blk [RR] \<^bold>r\<^bold>e\<^bold>s\<^bold>u\<^bold>l\<^bold>t\<^bold>s \<^bold>i\<^bold>n R\<heavy_comma> OBJ x \<Ztypecolon> Var var T)
       (Trueprop ((\<^bold>c\<^bold>u\<^bold>r\<^bold>r\<^bold>e\<^bold>n\<^bold>t blk [RR] \<^bold>r\<^bold>e\<^bold>s\<^bold>u\<^bold>l\<^bold>t\<^bold>s \<^bold>i\<^bold>n R\<heavy_comma> OBJ y \<Ztypecolon> Var var U) \<and> P))\<close>
   unfolding \<phi>Application_Method_def \<phi>Application_def
